yalla/fmformulas.v
@@ -16,14 +16,10 @@ Context { Atoms : AtomType_into_nat atom }.
 (** ** Encoding of [formula] into [nat]-labelled trees for ordering *)
 
 (** Embedding of [Atom] into [nat] *)
-Definition a2n := snd (proj1_sig Atom_into_nat).
-Definition n2a := fst (proj1_sig Atom_into_nat).
-Definition a2a_n : retract n2a a2n.
-Proof.
-unfold n2a, a2n.
-destruct Atom_into_nat as [(s, i) Hr].
-apply Hr.
-Defined.
+Notation a2n := (snd (proj1_sig Atom_into_nat)).
+Notation n2a := (fst (proj1_sig Atom_into_nat)).
+Definition a2a_n : retract n2a a2n :=
+  eq_rect _ _ (proj2_sig Atom_into_nat) _ (surjective_pairing (proj1_sig Atom_into_nat)).
 
 (** Embedding of [formula] into [nattree] *)
 Fixpoint form2nattree A :=
@@ -67,10 +63,9 @@ Proof. now intros A; induction A; cbn; rewrite ?IHA1, ?IHA2, ?IHA, ?a2a_n. Qed.
 
 #[export] Instance border_formula : BOrder | 50.
 Proof.
-eapply border_inj.
-eapply compose_injective.
+eapply border_inj, compose_injective.
 - eapply section_injective.
-  intros A; apply form_nattree_section.
+  intro; apply form_nattree_section.
 - apply nattree2nat_inj.
 Defined.
 
