yalla/ill_cut.v
@@ -26,11 +26,11 @@ Hypothesis P_gax_cut : forall a b l1 l2,
                           { c | l1 ++ fst (projT2 (ipgax P) a) ++ l2 = fst (projT2 (ipgax P) c)
                               & snd (projT2 (ipgax P) b) = snd (projT2 (ipgax P) c) }.
 
-Lemma cut_oc_comm_left (P_cutfree : ipcut P = false) n A C l1 l2 : ill P (l1 ++ ioc A :: l2) C ->
+Lemma cut_oc_comm_left (P_cutfree : ipcut P = false) n A C l1 l2 :
   (forall lw (pi0 : ill P (map ioc lw) A), ipsize pi0 < n -> ill P (l1 ++ map ioc lw ++ l2) C) ->
   forall l0 (pi1 : ill P l0 (ioc A)), ipsize pi1 <= n -> ill P (l1 ++ l0 ++ l2) C.
 Proof.
-intros pi2; induction n; intros IH l0 pi1 Hs;
+induction n; intros IH l0 pi1 Hs;
   remember (ioc A) as B; destruct_ill pi1 f X l Hl Hr HP a;
   try (now exfalso); try inversion HeqB.
 - apply (ex_ir (l1 ++ l ++ l2)).
@@ -42,147 +42,147 @@ intros pi2; induction n; intros IH l0 pi1 Hs;
   list_simpl; rewrite (app_assoc l), (app_assoc _ l0), <- (app_assoc l).
   cbn in Hs; refine (IHn _ _ Hl _); [ | lia ].
   intros; refine (IH _ pi0 _); lia.
-- list_simpl; rewrite app_assoc ; apply one_ilr.
+- list_simpl; rewrite app_assoc; apply one_ilr.
   list_simpl; rewrite (app_assoc l0).
   cbn in Hs; refine (IHn _ _ Hl _); [ | lia ].
   intros; refine (IH _ pi0 _); lia.
-- list_simpl; rewrite app_assoc ; apply tens_ilr.
-  list_simpl; rewrite 2 app_comm_cons ; rewrite (app_assoc l0).
+- list_simpl; rewrite app_assoc; apply tens_ilr.
+  list_simpl; rewrite 2 app_comm_cons, (app_assoc l0).
   cbn in Hs; refine (IHn _ _ Hl _); [ | lia ].
   intros; refine (IH _ pi0 _); lia.
-- list_simpl; rewrite app_assoc ; apply lpam_ilr; [ assumption | ].
-  list_simpl; rewrite app_comm_cons ; rewrite (app_assoc l3).
+- list_simpl; rewrite app_assoc; apply lpam_ilr; [ assumption | ].
+  list_simpl; rewrite app_comm_cons, (app_assoc l3).
   cbn in Hs; refine (IHn _ _ Hr _); [ | lia ].
   intros; refine (IH _ pi0 _); lia.
-- list_simpl; rewrite app_assoc ; apply lmap_ilr; [ assumption | ].
-  list_simpl; rewrite app_comm_cons ; rewrite (app_assoc l3).
+- list_simpl; rewrite app_assoc; apply lmap_ilr; [ assumption | ].
+  list_simpl; rewrite app_comm_cons, (app_assoc l3).
   cbn in Hs; refine (IHn _ _ Hr _); [ | lia ].
   intros; refine (IH _ pi0 _); lia.
-- list_simpl; rewrite app_assoc ; apply with_ilr1.
-  list_simpl; rewrite app_comm_cons ; rewrite (app_assoc l0).
+- list_simpl; rewrite app_assoc; apply with_ilr1.
+  list_simpl; rewrite app_comm_cons, (app_assoc l0).
   cbn in Hs; refine (IHn _ _ Hl _); [ | lia ].
   intros; refine (IH _ pi0 _); lia.
-- list_simpl; rewrite app_assoc ; apply with_ilr2.
-  list_simpl; rewrite app_comm_cons ; rewrite (app_assoc l0).
+- list_simpl; rewrite app_assoc; apply with_ilr2.
+  list_simpl; rewrite app_comm_cons, (app_assoc l0).
   cbn in Hs; refine (IHn _ _ Hl _); [ | lia ].
   intros; refine (IH _ pi0 _); lia.
-- list_simpl; rewrite app_assoc ; apply zero_ilr.
-- list_simpl; rewrite app_assoc ; apply plus_ilr.
-  + list_simpl; rewrite app_comm_cons ; rewrite (app_assoc l0).
+- list_simpl; rewrite app_assoc; apply zero_ilr.
+- list_simpl; rewrite app_assoc; apply plus_ilr.
+  + list_simpl; rewrite app_comm_cons, (app_assoc l0).
     cbn in Hs; refine (IHn _ _ Hl _); [ | lia ].
     intros; refine (IH _ pi0 _); lia.
-  + list_simpl; rewrite app_comm_cons ; rewrite (app_assoc l0).
+  + list_simpl; rewrite app_comm_cons, (app_assoc l0).
     cbn in Hs; refine (IHn _ _ Hr _); [ | lia ].
     intros; refine (IH _ pi0 _); lia.
 - subst; apply (IH _ Hl); cbn in Hs; lia.
-- list_simpl; rewrite app_assoc ; apply de_ilr.
-  list_simpl; rewrite app_comm_cons ; rewrite (app_assoc l0).
+- list_simpl; rewrite app_assoc; apply de_ilr.
+  list_simpl; rewrite app_comm_cons, (app_assoc l0).
   cbn in Hs; refine (IHn _ _ Hl _); [ | lia ].
   intros; refine (IH _ pi0 _); lia.
-- list_simpl; rewrite app_assoc ; apply wk_ilr.
+- list_simpl; rewrite app_assoc; apply wk_ilr.
   list_simpl; rewrite (app_assoc l0).
   cbn in Hs; refine (IHn _ _ Hl _); [ | lia ].
   intros; refine (IH _ pi0 _); lia.
-- list_simpl; rewrite app_assoc ; apply co_ilr.
-  list_simpl; rewrite 2 app_comm_cons ; rewrite (app_assoc l0).
+- list_simpl; rewrite app_assoc; apply co_ilr.
+  list_simpl; rewrite 2 app_comm_cons, (app_assoc l0).
   cbn in Hs; refine (IHn _ _ Hl _); [ | lia ].
   intros; refine (IH _ pi0 _); lia.
 - rewrite f in P_cutfree; inversion P_cutfree.
 - exfalso; assert (Hiq := P_gax_at_r a); rewrite H0 in Hiq; inversion Hiq.
 Qed.
 
-Lemma substitution_ioc : ipcut P = false -> forall A,
+Lemma substitution_ioc (P_cutfree : ipcut P = false) A :
   (forall l0 l1 l2 C, ill P l0 A -> ill P (l1 ++ A :: l2) C -> ill P (l1 ++ l0 ++ l2) C) ->
   forall lw l C, ill P (map ioc lw) A -> ill P l C -> forall l' L,
   l = l' ++ flat_map (cons (ioc A)) L -> ill P (l' ++ flat_map (app (map ioc lw)) L) C.
 Proof.
-intros P_cutfree A IHcut lw l C pi1 pi2.
-induction pi2 ; intros l' L Heq.
-- destruct l' ; inversion Heq.
-  + destruct L ; inversion Heq.
-  + symmetry in H1 ; apply app_eq_nil in H1 ; destruct H1 ; subst.
-    destruct L ; inversion H1.
+intros IHcut lw l C pi1 pi2.
+induction pi2; intros l' L Heq.
+- destruct l'; inversion Heq.
+  + destruct L; inversion Heq.
+  + symmetry in H1; apply app_eq_nil in H1; destruct H1; subst.
+    destruct L; inversion H1.
     apply ax_ir.
-- case_eq (ipperm P) ; intros Hperm ; rewrite Hperm in p ; cbn in p ; subst.
+- case_eq (ipperm P); intros Hperm; rewrite Hperm in p; cbn in p; subst.
   + destruct (Permutation_Type_app_flat_map_cst _ (map ioc lw) _ _ p)
       as [[L' l''] (Hnil' & HeqL' & HPL')];
-      cbn in Hnil' ; cbn in HeqL' ; cbn in HPL' ; subst.
-    eapply ex_ir ; [ | rewrite Hperm ; cbn ; apply HPL' ].
+      cbn in Hnil', HeqL', HPL'; subst.
+    eapply ex_ir; [ | rewrite Hperm; cbn; apply HPL' ].
     refine (IHpi2 _ _ _); reflexivity.
   + refine (IHpi2 _ _ _); reflexivity.
-- assert (injective (@ioc preiatom)) as Hinj by (intros x y Hxy ; inversion Hxy ; reflexivity).
+- assert (injective (@ioc preiatom)) as Hinj by (intros x y Hxy; inversion Hxy; reflexivity).
   destruct (Permutation_Type_flat_map_cons_flat_map_app_cst _ Hinj lw _ _ _ _ p Heq)
-    as [(((((lw1',lw2'),l1'),l2'),l''),L') HH] ; cbn in HH ; destruct HH as (H1 & H2 & H3 & H4).
-  rewrite <- H4 ; apply (ex_oc_ir _ lw1'); [ | assumption ].
-  rewrite H3 ; apply IHpi2; assumption.
-- symmetry in Heq ; apply app_eq_nil in Heq ; destruct Heq as [H Heq] ; subst.
-  destruct L ; inversion Heq.
+    as [(((((lw1',lw2'),l1'),l2'),l''),L') (H1 & H2 & H3 & H4)].
+  rewrite <- H4; apply (ex_oc_ir _ lw1'); [ | assumption ].
+  rewrite H3; apply IHpi2; assumption.
+- symmetry in Heq; apply app_eq_nil in Heq as [H Heq] ; subst.
+  destruct L; inversion Heq.
   apply one_irr.
 - elt_vs_app_flat_map_cst_inv Heq.
-  + list_simpl ; apply one_ilr.
-    rewrite app_assoc ; refine (IHpi2 _ _ _) ; list_simpl; reflexivity.
+  + list_simpl; apply one_ilr.
+    rewrite app_assoc; refine (IHpi2 _ _ _); list_simpl; reflexivity.
   + rewrite flat_map_app.
-    list_simpl ; rewrite 3 app_assoc ; apply one_ilr.
+    list_simpl; rewrite 3 app_assoc; apply one_ilr.
     rewrite <- 3 app_assoc.
     replace (map ioc lw ++ l ++ l0 ++ flat_map (app (map ioc lw)) L1)
-       with (flat_map (app (map ioc lw)) ((l ++ l0) :: L1)) by (list_simpl ; reflexivity).
-    rewrite <- flat_map_app ; refine (IHpi2 _ _ _).
-    rewrite ? flat_map_app ; list_simpl; reflexivity.
+       with (flat_map (app (map ioc lw)) ((l ++ l0) :: L1)) by (list_simpl; reflexivity).
+    rewrite <- flat_map_app; refine (IHpi2 _ _ _).
+    rewrite ? flat_map_app; list_simpl; reflexivity.
 - app_vs_app_flat_map_cst_inv Heq.
-  + list_simpl ; apply tens_irr; [ assumption | ].
+  + list_simpl; apply tens_irr; [ assumption | ].
     refine (IHpi2_2 _ _ _); reflexivity.
-  + rewrite flat_map_app ; list_simpl.
-    rewrite 3 app_assoc ; apply tens_irr.
+  + rewrite flat_map_app; list_simpl.
+    rewrite 3 app_assoc; apply tens_irr.
     * list_simpl.
       replace (flat_map (app (map ioc lw)) L0 ++ map ioc lw ++ l)
          with (flat_map (app (map ioc lw)) (L0 ++ l :: nil))
-        by (rewrite flat_map_app ; list_simpl ; reflexivity).
+        by (rewrite flat_map_app; list_simpl; reflexivity).
       refine (IHpi2_1 _ _ _); reflexivity.
     * refine (IHpi2_2 _ _ _); reflexivity.
-  + rewrite flat_map_app ; list_simpl.
-    rewrite app_assoc ; apply tens_irr.
+  + rewrite flat_map_app; list_simpl.
+    rewrite app_assoc; apply tens_irr.
     * refine (IHpi2_1 _ _ _); reflexivity.
     * rewrite <- (app_nil_l _) ; refine (IHpi2_2 _ _ _); reflexivity.
 - elt_vs_app_flat_map_cst_inv Heq.
-  + list_simpl ; apply tens_ilr.
-    rewrite 2 app_comm_cons ; rewrite app_assoc ; refine (IHpi2 _ _ _) ; list_simpl; reflexivity.
+  + list_simpl; apply tens_ilr.
+    rewrite 2 app_comm_cons, app_assoc; refine (IHpi2 _ _ _); list_simpl; reflexivity.
   + rewrite flat_map_app.
-    list_simpl ; rewrite 3 app_assoc ; apply tens_ilr.
+    list_simpl; rewrite 3 app_assoc; apply tens_ilr.
     rewrite <- 3 app_assoc.
     replace (map ioc lw ++ l ++ A0 :: B :: l0 ++ flat_map (app (map ioc lw)) L1)
-      with (flat_map (app (map ioc lw)) ((l ++ A0 :: B :: l0) :: L1)) by (list_simpl ; reflexivity).
-    rewrite <- flat_map_app ; refine (IHpi2 _ _ _).
-    rewrite ? flat_map_app ; list_simpl; reflexivity.
+      with (flat_map (app (map ioc lw)) ((l ++ A0 :: B :: l0) :: L1)) by (list_simpl; reflexivity).
+    rewrite <- flat_map_app; refine (IHpi2 _ _ _).
+    rewrite ? flat_map_app; list_simpl; reflexivity.
 - apply lpam_irr.
-  induction L using rev_rect ; list_simpl.
+  induction L using rev_rect; list_simpl.
   + change nil with (nil ++ flat_map (app (map ioc lw)) nil).
     rewrite app_comm_cons, app_assoc; refine (IHpi2 _ _ _); subst; list_simpl; reflexivity.
   + replace (flat_map (app (map ioc lw)) L ++ map ioc lw ++ x ++ A0 :: nil)
        with (flat_map (app (map ioc lw)) (L ++ (x ++ (A0 :: nil)) :: nil))
       by now list_simpl.
-    refine (IHpi2 _ _ _) ; subst ; list_simpl; reflexivity.
+    refine (IHpi2 _ _ _); subst; list_simpl; reflexivity.
 - elt_vs_app_flat_map_cst_inv Heq.
   + app_vs_app_flat_map_cst_inv Heq1.
-    * list_simpl ; apply lpam_ilr; [ assumption | ].
+    * list_simpl; apply lpam_ilr; [ assumption | ].
       rewrite app_comm_cons, app_assoc; refine (IHpi2_2 _ _ _); list_simpl; reflexivity.
-    * list_simpl ; rewrite ? flat_map_app ; list_simpl.
-      rewrite (app_assoc l) ; rewrite (app_assoc _ (map ioc lw)) ; rewrite (app_assoc _ l3).
+    * list_simpl; rewrite ? flat_map_app; list_simpl.
+      rewrite (app_assoc l), (app_assoc _ (map ioc lw)), (app_assoc _ l3).
       replace (((l ++ flat_map (app (map ioc lw)) L0) ++ map ioc lw) ++ l3)
          with (l ++ flat_map (app (map ioc lw)) (L0 ++ l3 :: nil))
-        by (rewrite flat_map_app ; list_simpl ; reflexivity).
+        by (rewrite flat_map_app; list_simpl; reflexivity).
       apply lpam_ilr.
       -- refine (IHpi2_1 _ _ _); reflexivity.
       -- rewrite app_comm_cons, app_assoc; refine (IHpi2_2 _ _ _); list_simpl; reflexivity.
-    * list_simpl; rewrite (app_assoc l) ; apply lpam_ilr.
+    * list_simpl; rewrite (app_assoc l); apply lpam_ilr.
       -- refine (IHpi2_1 _ _ _); reflexivity.
       -- rewrite <- (app_nil_l (flat_map _ _)), app_comm_cons, app_assoc;
            refine (IHpi2_2 _ _ _); list_simpl; reflexivity.
   + app_vs_app_flat_map_cst_inv Heq2.
-    * list_simpl ; rewrite ? flat_map_app ; list_simpl.
-      rewrite (app_assoc l') ; rewrite (app_assoc _ (map ioc lw)) ; rewrite (app_assoc _ l).
+    * list_simpl; rewrite ? flat_map_app; list_simpl.
+      rewrite (app_assoc l'), (app_assoc _ (map ioc lw)), (app_assoc _ l).
       replace (((l' ++ flat_map (app (map ioc lw)) L0) ++ map ioc lw) ++ l)
          with (l' ++ flat_map (app (map ioc lw)) (L0 ++ l :: nil))
-        by (rewrite flat_map_app ; list_simpl ; reflexivity).
+        by (rewrite flat_map_app; list_simpl; reflexivity).
       apply lpam_ilr; [ assumption | ].
       list_simpl.
       replace (flat_map (app (map ioc lw)) L0 ++ map ioc lw ++ l ++
@@ -193,51 +193,50 @@ induction pi2 ; intros l' L Heq.
     * list_simpl; rewrite (app_assoc l3), (app_assoc _ _ (l1 ++ _)), (app_assoc _ l1).
       replace (((l3 ++ flat_map (app (map ioc lw)) L) ++ map ioc lw) ++ l1)
          with (l3 ++ flat_map (app (map ioc lw)) (L ++ l1 :: nil))
-        by (rewrite flat_map_app ; list_simpl ; reflexivity).
-      rewrite 3 app_assoc ; apply lpam_ilr.
+        by (rewrite flat_map_app; list_simpl; reflexivity).
+      rewrite 3 app_assoc; apply lpam_ilr.
       -- refine (IHpi2_1 _ _ _); reflexivity.
       -- list_simpl.
          replace (flat_map (app (map ioc lw)) L0 ++ map ioc lw ++ l ++ B :: l4
                                                  ++ flat_map (app (map ioc lw)) L2)
             with (flat_map (app (map ioc lw)) (L0 ++ (l ++ B :: l4) :: L2))
            by (rewrite ? flat_map_app ; list_simpl ; reflexivity).
-         refine (IHpi2_2 _ _ _) ; rewrite ? flat_map_app ; list_simpl; reflexivity.
-    * list_simpl ; rewrite ? flat_map_app ; list_simpl ; rewrite ? flat_map_app ; list_simpl.
-      rewrite (app_assoc l3) ; rewrite 3 app_assoc ; apply lpam_ilr.
+         refine (IHpi2_2 _ _ _); rewrite ? flat_map_app; list_simpl; reflexivity.
+    * list_simpl; rewrite ? flat_map_app; list_simpl; rewrite ? flat_map_app; list_simpl.
+      rewrite (app_assoc l3), 3 app_assoc; apply lpam_ilr.
       -- refine (IHpi2_1 _ _ _); reflexivity.
       -- list_simpl.
          replace (flat_map (app (map ioc lw)) L0 ++ map ioc lw ++ l
                                                  ++ B :: flat_map (app (map ioc lw)) L2)
             with (flat_map (app (map ioc lw)) (L0 ++ (l ++ B :: nil) :: L2))
-           by (rewrite ? flat_map_app ; list_simpl ; reflexivity).
-         refine (IHpi2_2 _ _ _) ; rewrite ? flat_map_app ; list_simpl; reflexivity.
+           by (rewrite ? flat_map_app; list_simpl; reflexivity).
+         refine (IHpi2_2 _ _ _); rewrite ? flat_map_app; list_simpl; reflexivity.
 - apply gen_irr.
-  induction L using rev_rect ; list_simpl.
+  induction L using rev_rect; list_simpl.
   + change nil with (nil ++ flat_map (app (map ioc lw)) nil).
     rewrite app_comm_cons, app_assoc; refine (IHpi2 _ _ _); subst; list_simpl; reflexivity.
   + replace (flat_map (app (map ioc lw)) L ++ map ioc lw ++ x ++ A0 :: nil)
        with (flat_map (app (map ioc lw)) (L ++ (x ++ (A0 :: nil)) :: nil))
       by now list_simpl.
-    refine (IHpi2 _ _ _) ; subst ; list_simpl; reflexivity.
-- destruct l' ; inversion Heq ; subst.
-  + destruct L ; inversion H0.
+    refine (IHpi2 _ _ _); subst; list_simpl; reflexivity.
+- destruct l' ; inversion Heq; subst.
+  + destruct L; inversion H0.
   + list_simpl.
-    apply gen_ilr.
-    apply IHpi2; reflexivity.
+    apply gen_ilr, IHpi2; reflexivity.
 - apply lmap_irr.
-  rewrite app_comm_cons ; refine (IHpi2 _ _ _) ; subst ; list_simpl; reflexivity.
+  rewrite app_comm_cons; refine (IHpi2 _ _ _); subst; list_simpl; reflexivity.
 - rewrite app_assoc in Heq; elt_vs_app_flat_map_cst_inv Heq.
-  + list_simpl ; apply lmap_ilr; [ assumption | ].
+  + list_simpl; apply lmap_ilr; [ assumption | ].
     rewrite app_comm_cons, app_assoc; refine (IHpi2_2 _ _ _); list_simpl; reflexivity.
   + replace (flat_map (cons (ioc A)) L0 ++ ioc A :: l)
        with (flat_map (cons (ioc A)) (L0 ++ l :: nil))
-      in Heq1 by (rewrite flat_map_app ; list_simpl ; reflexivity).
+      in Heq1 by (rewrite flat_map_app; list_simpl; reflexivity).
     app_vs_app_flat_map_cst_inv Heq1.
-    * list_simpl ; rewrite ? flat_map_app ; list_simpl.
-      rewrite (app_assoc l2) ; rewrite (app_assoc _ (map ioc lw)) ; rewrite (app_assoc _ l).
+    * list_simpl; rewrite ? flat_map_app; list_simpl.
+      rewrite (app_assoc l2), (app_assoc _ (map ioc lw)), (app_assoc _ l).
       replace (((l2 ++ flat_map (app (map ioc lw)) L0) ++ map ioc lw) ++ l)
          with (l2 ++ flat_map (app (map ioc lw)) (L0 ++ l :: nil))
-        by (rewrite flat_map_app ; list_simpl ; reflexivity).
+        by (rewrite flat_map_app; list_simpl; reflexivity).
       apply lmap_ilr.
       -- refine (IHpi2_1 _ _ _); reflexivity.
       -- rewrite app_comm_cons, app_assoc; refine (IHpi2_2 _ _ _); list_simpl; reflexivity.
@@ -245,250 +244,250 @@ induction pi2 ; intros l' L Heq.
       -- assert (L0 = L /\ l = l2 ++ l4) as [Heq1 Heq2] ; subst.
          { apply (f_equal (@rev _)) in Heq0.
            rewrite ? rev_app_distr in Heq0.
-           inversion Heq0 ; subst.
+           inversion Heq0; subst.
            apply (f_equal (@rev _)) in H1.
-           rewrite ? rev_involutive in H1 ; subst.
+           rewrite ? rev_involutive in H1; subst.
            split; reflexivity. }
-         list_simpl ; rewrite ? flat_map_app ; list_simpl ; rewrite ? flat_map_app ; list_simpl.
+         list_simpl; rewrite ? flat_map_app; list_simpl; rewrite ? flat_map_app; list_simpl.
          list_simpl in pi2_1.
-         rewrite 3 app_assoc ; apply lmap_ilr; [ assumption | ].
-         list_simpl ; rewrite <- app_assoc in IHpi2_2.
+         rewrite 3 app_assoc; apply lmap_ilr; [ assumption | ].
+         list_simpl; rewrite <- app_assoc in IHpi2_2.
          replace (flat_map (cons (ioc A)) (L ++ l2 :: nil) ++ B :: l3 ++ flat_map (cons (ioc A)) L1)
             with (flat_map (cons (ioc A)) (L ++ (l2 ++ B :: l3) :: L1)) in IHpi2_2
-           by (rewrite ? flat_map_app ; list_simpl ; reflexivity).
+           by (rewrite ? flat_map_app; list_simpl; reflexivity).
          assert (pi2' := IHpi2_2 _ _ eq_refl).
-         rewrite ? flat_map_app in pi2' ; list_simpl in pi2'; assumption.
-      -- assert (L0 = L ++ (l2 ++ l4) :: L2 /\ l = x) as [Heq1 Heq2] ; subst.
+         rewrite ? flat_map_app in pi2'; list_simpl in pi2'; assumption.
+      -- assert (L0 = L ++ (l2 ++ l4) :: L2 /\ l = x) as [Heq1 Heq2]; subst.
          { apply (f_equal (@rev _)) in Heq0.
-           rewrite ? rev_app_distr in Heq0 ; list_simpl in Heq0.
-           inversion Heq0 ; subst.
+           rewrite ? rev_app_distr in Heq0; list_simpl in Heq0.
+           inversion Heq0; subst.
            apply (f_equal (@rev _)) in H1.
-           rewrite ? rev_involutive in H1 ; subst.
-           rewrite ? rev_app_distr ; list_simpl ; split; reflexivity. }
-         list_simpl ; rewrite ? flat_map_app ; list_simpl ; rewrite ? flat_map_app ; list_simpl.
+           rewrite ? rev_involutive in H1; subst.
+           rewrite ? rev_app_distr; list_simpl; split; reflexivity. }
+         list_simpl; rewrite ? flat_map_app; list_simpl; rewrite ? flat_map_app; list_simpl.
          rewrite 3 app_assoc, (app_assoc l4), (app_assoc (l4 ++ _)), (app_assoc _ x).
          apply lmap_ilr.
          ++ list_simpl.
             replace (flat_map (app (map ioc lw)) L2 ++ map ioc lw ++ x)
                with (flat_map (app (map ioc lw)) (L2 ++ x :: nil))
-              by (rewrite flat_map_app ; list_simpl ; reflexivity).
+              by (rewrite flat_map_app; list_simpl; reflexivity).
             refine (IHpi2_1 _ _ _); reflexivity.
-         ++ list_simpl ; rewrite <- app_assoc in IHpi2_2.
+         ++ list_simpl; rewrite <- app_assoc in IHpi2_2.
             replace (flat_map (cons (ioc A)) (L ++ l2 :: nil) ++
                        B :: l3 ++ flat_map (cons (ioc A)) L1)
                with (flat_map (cons (ioc A)) (L ++ (l2 ++ B :: l3) :: L1)) in IHpi2_2
-              by (rewrite ? flat_map_app ; list_simpl ; reflexivity).
+              by (rewrite ? flat_map_app; list_simpl; reflexivity).
             assert (pi2' := IHpi2_2 _ _ eq_refl).
-            rewrite ? flat_map_app in pi2' ; list_simpl in pi2'; assumption.
-    * induction L2 using rev_rect ; [ | clear IHL2 ].
-      -- list_simpl in Heq0 ; subst.
-         list_simpl ; rewrite ? flat_map_app ; list_simpl ; rewrite ? flat_map_app ; list_simpl.
+            rewrite ? flat_map_app in pi2'; list_simpl in pi2'; assumption.
+    * induction L2 using rev_rect; [ | clear IHL2 ].
+      -- list_simpl in Heq0; subst.
+         list_simpl; rewrite ? flat_map_app; list_simpl; rewrite ? flat_map_app; list_simpl.
          list_simpl in pi2_1.
          rewrite <- (app_nil_l (ilmap _ _ :: _)), 3 app_assoc; apply lmap_ilr; [ assumption | ].
-         list_simpl ; rewrite <- app_assoc in IHpi2_2.
+         list_simpl; rewrite <- app_assoc in IHpi2_2.
          replace (flat_map (cons (ioc A)) (L0 ++ l :: nil) ++ B :: l3 ++ flat_map (cons (ioc A)) L1)
             with (flat_map (cons (ioc A)) (L0 ++ (l ++ B :: l3) :: L1)) in IHpi2_2
-           by (rewrite ? flat_map_app ; list_simpl ; reflexivity).
+           by (rewrite ? flat_map_app; list_simpl; reflexivity).
          assert (pi2' := IHpi2_2 _ _ eq_refl).
-         rewrite ? flat_map_app in pi2' ; list_simpl in pi2'; assumption.
+         rewrite ? flat_map_app in pi2'; list_simpl in pi2'; assumption.
       -- assert (L0 = L ++ L2 /\ l = x) as [Heq1 Heq2] ; subst.
          { apply (f_equal (@rev _)) in Heq0.
-           rewrite ? rev_app_distr in Heq0 ; list_simpl in Heq0.
-           inversion Heq0 ; subst.
+           rewrite ? rev_app_distr in Heq0; list_simpl in Heq0.
+           inversion Heq0; subst.
            apply (f_equal (@rev _)) in H1.
-           rewrite rev_involutive in H1 ; subst.
-           rewrite rev_app_distr ; list_simpl ; split; reflexivity. }
-         list_simpl ; rewrite ? flat_map_app ; list_simpl ; rewrite ? flat_map_app ; list_simpl.
+           rewrite rev_involutive in H1; subst.
+           rewrite rev_app_distr; list_simpl; split; reflexivity. }
+         list_simpl; rewrite ? flat_map_app; list_simpl; rewrite ? flat_map_app; list_simpl.
          rewrite app_assoc, (app_assoc _ (map ioc lw)), (app_assoc _ x); apply lmap_ilr.
          ++ list_simpl.
             replace (flat_map (app (map ioc lw)) L2 ++ map ioc lw ++ x)
                with (flat_map (app (map ioc lw)) (L2 ++ x :: nil))
-              by (rewrite flat_map_app ; list_simpl ; reflexivity).
+              by (rewrite flat_map_app; list_simpl; reflexivity).
             rewrite <- (app_nil_l _).
             refine (IHpi2_1 _ _ _); reflexivity.
-         ++ induction L using rev_rect ; [ | clear IHL ].
-            ** list_simpl in IHpi2_2 ; list_simpl.
+         ++ induction L using rev_rect; [ | clear IHL ].
+            ** list_simpl in IHpi2_2; list_simpl.
                rewrite app_comm_cons, app_assoc; refine (IHpi2_2 _ _ _); list_simpl; reflexivity.
-            ** list_simpl ; rewrite <- app_assoc in IHpi2_2.
+            ** list_simpl; rewrite <- app_assoc in IHpi2_2.
                replace (flat_map (cons (ioc A)) (L ++ x0 :: nil) ++
                           B :: l3 ++ flat_map (cons (ioc A)) L1)
                   with (flat_map (cons (ioc A)) (L ++ (x0 ++ B :: l3) :: L1)) in IHpi2_2
-                 by (rewrite ? flat_map_app ; list_simpl ; reflexivity).
+                 by (rewrite ? flat_map_app; list_simpl; reflexivity).
                assert (pi2' := IHpi2_2 _ _ eq_refl).
-               rewrite ? flat_map_app in pi2' ; list_simpl in pi2'.
-               rewrite ? flat_map_app ; list_simpl; assumption.
+               rewrite ? flat_map_app in pi2'; list_simpl in pi2'.
+               rewrite ? flat_map_app; list_simpl; assumption.
 - apply neg_irr.
-  rewrite app_comm_cons ; refine (IHpi2 _ _ _) ; subst ; list_simpl; reflexivity.
+  rewrite app_comm_cons; refine (IHpi2 _ _ _); subst; list_simpl; reflexivity.
 - elt_vs_app_flat_map_cst_inv Heq.
-  + symmetry in Heq1 ; apply app_eq_nil in Heq1 ; destruct Heq1 as [Heq Heq1] ; subst.
-    destruct L ; inversion Heq1.
-    list_simpl ; apply neg_ilr; assumption.
-  + symmetry in Heq2 ; apply app_eq_nil in Heq2 ; destruct Heq2 as [Heq Heq2] ; subst.
-    destruct L1 ; inversion Heq2.
+  + symmetry in Heq1; apply app_eq_nil in Heq1 as [-> Heq1].
+    destruct L; inversion Heq1.
+    list_simpl; apply neg_ilr; assumption.
+  + symmetry in Heq2; apply app_eq_nil in Heq2 as [Heq Heq2]; subst.
+    destruct L1; inversion Heq2.
     rewrite flat_map_app.
-    list_simpl ; rewrite 3 app_assoc ; apply neg_ilr.
+    list_simpl; rewrite 3 app_assoc; apply neg_ilr.
     rewrite <- 2 app_assoc.
     replace (map ioc lw ++ l0)
-      with (flat_map (app (map ioc lw)) (l0 :: nil)) by (list_simpl ; reflexivity).
-    rewrite <- flat_map_app ; refine (IHpi2 _ _ _).
-    rewrite ? flat_map_app ; list_simpl; reflexivity.
+      with (flat_map (app (map ioc lw)) (l0 :: nil)) by (list_simpl; reflexivity).
+    rewrite <- flat_map_app; refine (IHpi2 _ _ _).
+    rewrite ? flat_map_app; list_simpl; reflexivity.
 - apply top_irr.
 - apply with_irr.
-  + refine (IHpi2_1 _ _ _) ; list_simpl; assumption.
-  + refine (IHpi2_2 _ _ _) ; list_simpl; assumption.
+  + refine (IHpi2_1 _ _ _); list_simpl; assumption.
+  + refine (IHpi2_2 _ _ _); list_simpl; assumption.
 - elt_vs_app_flat_map_cst_inv Heq.
-  + list_simpl ; apply with_ilr1.
+  + list_simpl; apply with_ilr1.
     rewrite app_comm_cons, app_assoc; refine (IHpi2 _ _ _); list_simpl; reflexivity.
   + rewrite flat_map_app.
-    list_simpl ; rewrite 3 app_assoc ; apply with_ilr1.
+    list_simpl; rewrite 3 app_assoc; apply with_ilr1.
     rewrite <- 3 app_assoc.
     replace (map ioc lw ++ l ++ A0 :: l0 ++ flat_map (app (map ioc lw)) L1)
-      with (flat_map (app (map ioc lw)) ((l ++ A0 :: l0) :: L1)) by (list_simpl ; reflexivity).
-    rewrite <- flat_map_app ; refine (IHpi2 _ _ _).
-    rewrite ? flat_map_app ; list_simpl; reflexivity.
+      with (flat_map (app (map ioc lw)) ((l ++ A0 :: l0) :: L1)) by (list_simpl; reflexivity).
+    rewrite <- flat_map_app; refine (IHpi2 _ _ _).
+    rewrite ? flat_map_app; list_simpl; reflexivity.
 - elt_vs_app_flat_map_cst_inv Heq.
-  + list_simpl ; apply with_ilr2.
+  + list_simpl; apply with_ilr2.
     rewrite app_comm_cons, app_assoc; refine (IHpi2 _ _ _); list_simpl; reflexivity.
   + rewrite flat_map_app.
-    list_simpl ; rewrite 3 app_assoc ; apply with_ilr2.
+    list_simpl; rewrite 3 app_assoc; apply with_ilr2.
     rewrite <- 3 app_assoc.
     replace (map ioc lw ++ l ++ A0 :: l0 ++ flat_map (app (map ioc lw)) L1)
-      with (flat_map (app (map ioc lw)) ((l ++ A0 :: l0) :: L1)) by (list_simpl ; reflexivity).
-    rewrite <- flat_map_app ; refine (IHpi2 _ _ _).
-    rewrite ? flat_map_app ; list_simpl; reflexivity.
+      with (flat_map (app (map ioc lw)) ((l ++ A0 :: l0) :: L1)) by (list_simpl; reflexivity).
+    rewrite <- flat_map_app; refine (IHpi2 _ _ _).
+    rewrite ? flat_map_app; list_simpl; reflexivity.
 - elt_vs_app_flat_map_cst_inv Heq.
-  + list_simpl ; apply zero_ilr.
+  + list_simpl; apply zero_ilr.
   + rewrite flat_map_app.
-    list_simpl ; rewrite 3 app_assoc ; apply zero_ilr.
+    list_simpl; rewrite 3 app_assoc; apply zero_ilr.
 - apply plus_irr1.
-  refine (IHpi2 _ _ _) ; subst ; list_simpl; reflexivity.
+  refine (IHpi2 _ _ _); subst; list_simpl; reflexivity.
 - apply plus_irr2.
-  refine (IHpi2 _ _ _) ; subst ; list_simpl; reflexivity.
+  refine (IHpi2 _ _ _); subst; list_simpl; reflexivity.
 - elt_vs_app_flat_map_cst_inv Heq.
-  + list_simpl ; apply plus_ilr.
+  + list_simpl; apply plus_ilr.
     * rewrite app_comm_cons, app_assoc; refine (IHpi2_1 _ _ _); list_simpl; reflexivity.
     * rewrite app_comm_cons, app_assoc; refine (IHpi2_2 _ _ _); list_simpl; reflexivity.
   + rewrite flat_map_app.
-    list_simpl ; rewrite 3 app_assoc ; apply plus_ilr ; rewrite <- 3 app_assoc.
+    list_simpl; rewrite 3 app_assoc; apply plus_ilr; rewrite <- 3 app_assoc.
     * replace (map ioc lw ++ l ++ A0 :: l0 ++ flat_map (app (map ioc lw)) L1)
-        with (flat_map (app (map ioc lw)) ((l ++ A0 :: l0) :: L1)) by (list_simpl ; reflexivity).
-      rewrite <- flat_map_app ; refine (IHpi2_1 _ _ _).
-      rewrite ? flat_map_app ; list_simpl; reflexivity.
+        with (flat_map (app (map ioc lw)) ((l ++ A0 :: l0) :: L1)) by (list_simpl; reflexivity).
+      rewrite <- flat_map_app; refine (IHpi2_1 _ _ _).
+      rewrite ? flat_map_app; list_simpl; reflexivity.
     * replace (map ioc lw ++ l ++ B :: l0 ++ flat_map (app (map ioc lw)) L1)
-        with (flat_map (app (map ioc lw)) ((l ++ B :: l0) :: L1)) by (list_simpl ; reflexivity).
-      rewrite <- flat_map_app ; refine (IHpi2_2 _ _ _).
-      rewrite ? flat_map_app ; list_simpl; reflexivity.
+        with (flat_map (app (map ioc lw)) ((l ++ B :: l0) :: L1)) by (list_simpl; reflexivity).
+      rewrite <- flat_map_app; refine (IHpi2_2 _ _ _).
+      rewrite ? flat_map_app; list_simpl; reflexivity.
 - decomp_map_inf Heq; subst; cbn in Heq2; cbn.
   assert ({ Lw | flat_map (app (map ioc lw)) L = map ioc Lw }) as [Lw HeqLw].
   { clear pi2 IHpi2 ; revert l2 Heq2 ; clear ; induction L ; intros l2 Heq2.
     - exists nil; reflexivity.
     - cbn in Heq2.
-      decomp_map_inf Heq2 ; subst.
-      inversion Heq1 ; subst ; cbn.
-      cbn in Heq4 ; apply IHL in Heq4.
-      destruct Heq4 as [Lw Heq4].
-      exists (lw ++ l1 ++ Lw) ; list_simpl ; rewrite <- Heq4; reflexivity. }
-  rewrite HeqLw ; rewrite <- map_app ; apply oc_irr.
-  list_simpl ; rewrite <- HeqLw ; refine (IHpi2 _ _ _).
+      decomp_map_inf Heq2; subst.
+      inversion Heq1; subst; cbn.
+      cbn in Heq4; apply IHL in Heq4 as [Lw Heq4].
+      exists (lw ++ l1 ++ Lw); list_simpl; rewrite <- Heq4; reflexivity. }
+  rewrite HeqLw, <- map_app; apply oc_irr.
+  list_simpl; rewrite <- HeqLw; refine (IHpi2 _ _ _).
   rewrite <- Heq2; list_simpl; reflexivity.
 - elt_vs_app_flat_map_cst_inv Heq.
-  + list_simpl ; apply de_ilr.
+  + list_simpl; apply de_ilr.
     rewrite app_comm_cons, app_assoc; refine (IHpi2 _ _ _); list_simpl; reflexivity.
   + rewrite flat_map_app.
-    list_simpl ; rewrite 3 app_assoc ; apply de_ilr.
+    list_simpl; rewrite 3 app_assoc; apply de_ilr.
     rewrite <- 3 app_assoc.
     replace (map ioc lw ++ l ++ A0 :: l0 ++ flat_map (app (map ioc lw)) L1)
-      with (flat_map (app (map ioc lw)) ((l ++ A0 :: l0) :: L1)) by (list_simpl ; reflexivity).
-    rewrite <- flat_map_app ; refine (IHpi2 _ _ _).
-    rewrite ? flat_map_app ; list_simpl; reflexivity.
-  + inversion HeqA ; subst.
-    induction L0 using rev_rect ; [ | clear IHL0 ].
-    * list_simpl ; list_simpl in IHpi2.
-      rewrite app_comm_cons in IHpi2 ; rewrite app_assoc in IHpi2.
+      with (flat_map (app (map ioc lw)) ((l ++ A0 :: l0) :: L1)) by (list_simpl; reflexivity).
+    rewrite <- flat_map_app; refine (IHpi2 _ _ _).
+    rewrite ? flat_map_app; list_simpl; reflexivity.
+  + inversion HeqA; subst.
+    induction L0 using rev_rect; [ | clear IHL0 ].
+    * list_simpl; list_simpl in IHpi2.
+      rewrite app_comm_cons, app_assoc in IHpi2.
       assert (pi2' := IHpi2 _ _ eq_refl).
-      list_simpl in pi2' ; apply (IHcut _ _ _ _ pi1) in pi2'; assumption.
+      list_simpl in pi2'; apply (IHcut _ _ _ _ pi1) in pi2'; assumption.
     * rewrite <- ? app_assoc in IHpi2.
       replace (flat_map (cons (ioc A)) (L0 ++ x :: nil) ++ A :: l ++ flat_map (cons (ioc A)) L1)
          with (flat_map (cons (ioc A)) (L0 ++ (x ++ A :: l) :: L1)) in IHpi2
-        by (rewrite ? flat_map_app ; list_simpl ; reflexivity).
+        by (rewrite ? flat_map_app; list_simpl; reflexivity).
       assert (pi2' := IHpi2 _ _ eq_refl).
-      rewrite flat_map_app in pi2' ; list_simpl in pi2'.
-      rewrite 3 app_assoc in pi2' ; apply (IHcut _ _ _ _ pi1) in pi2'.
-      list_simpl in pi2' ; rewrite ? flat_map_app ; list_simpl; assumption.
+      rewrite flat_map_app in pi2'; list_simpl in pi2'.
+      rewrite 3 app_assoc in pi2'; apply (IHcut _ _ _ _ pi1) in pi2'.
+      list_simpl in pi2'; rewrite ? flat_map_app; list_simpl; assumption.
 - elt_vs_app_flat_map_cst_inv Heq.
-  + list_simpl ; apply wk_ilr.
-    rewrite app_assoc ; refine (IHpi2 _ _ _) ; list_simpl; reflexivity.
+  + list_simpl; apply wk_ilr.
+    rewrite app_assoc; refine (IHpi2 _ _ _); list_simpl; reflexivity.
   + rewrite flat_map_app.
-    list_simpl ; rewrite 3 app_assoc ; apply wk_ilr.
+    list_simpl; rewrite 3 app_assoc; apply wk_ilr.
     rewrite <- 3 app_assoc.
     replace (map ioc lw ++ l ++ l0 ++ flat_map (app (map ioc lw)) L1)
       with (flat_map (app (map ioc lw)) ((l ++ l0) :: L1)) by (list_simpl ; reflexivity).
-    rewrite <- flat_map_app ; refine (IHpi2 _ _ _).
-    rewrite ? flat_map_app ; list_simpl; reflexivity.
-  + inversion HeqA ; subst.
-    induction L0 using rev_rect ; [ | clear IHL0 ].
-    * list_simpl ; apply wk_list_ilr.
-      list_simpl in IHpi2 ; rewrite app_assoc in IHpi2.
-      rewrite app_assoc ; refine (IHpi2 _ _ _); reflexivity.
+    rewrite <- flat_map_app; refine (IHpi2 _ _ _).
+    rewrite ? flat_map_app; list_simpl; reflexivity.
+  + inversion HeqA; subst.
+    induction L0 using rev_rect; [ | clear IHL0 ].
+    * list_simpl; apply wk_list_ilr.
+      list_simpl in IHpi2; rewrite app_assoc in IHpi2.
+      rewrite app_assoc; refine (IHpi2 _ _ _); reflexivity.
     * rewrite <- ? app_assoc in IHpi2.
       replace (flat_map (cons (ioc A)) (L0 ++ x :: nil) ++ l ++ flat_map (cons (ioc A)) L1)
          with (flat_map (cons (ioc A)) (L0 ++ (x ++ l) :: L1)) in IHpi2
-        by (rewrite ? flat_map_app ; list_simpl ; reflexivity).
+        by (rewrite ? flat_map_app; list_simpl; reflexivity).
       assert (pi2' := IHpi2 _ _ eq_refl).
       list_simpl in pi2'; list_simpl.
-      rewrite 3 app_assoc ; apply wk_list_ilr ; list_simpl; assumption.
+      rewrite 3 app_assoc; apply wk_list_ilr; list_simpl; assumption.
 - elt_vs_app_flat_map_cst_inv Heq.
-  + list_simpl ; apply co_ilr.
+  + list_simpl; apply co_ilr.
     rewrite 2 app_comm_cons, app_assoc; refine (IHpi2 _ _ _); list_simpl; reflexivity.
   + rewrite flat_map_app.
-    list_simpl ; rewrite 3 app_assoc ; apply co_ilr.
+    list_simpl; rewrite 3 app_assoc; apply co_ilr.
     rewrite <- 3 app_assoc.
     replace (map ioc lw ++ l ++ ioc A0 :: ioc A0 :: l0 ++ flat_map (app (map ioc lw)) L1)
       with (flat_map (app (map ioc lw)) ((l ++ ioc A0 :: ioc A0 :: l0) :: L1))
       by (list_simpl; reflexivity).
-    rewrite <- flat_map_app ; refine (IHpi2 _ _ _).
-    rewrite ? flat_map_app ; list_simpl; reflexivity.
-  + inversion HeqA ; subst.
-    induction L0 using rev_rect ; [ | clear IHL0 ].
-    * list_simpl ; apply co_list_ilr.
+    rewrite <- flat_map_app; refine (IHpi2 _ _ _).
+    rewrite ? flat_map_app; list_simpl; reflexivity.
+  + inversion HeqA; subst.
+    induction L0 using rev_rect; [ | clear IHL0 ].
+    * list_simpl; apply co_list_ilr.
       list_simpl in IHpi2.
       replace (ioc A :: ioc A :: l ++ flat_map (cons (ioc A)) L1)
          with (flat_map (cons (ioc A)) (nil :: l :: L1)) in IHpi2
-        by (list_simpl ; reflexivity).
+        by (list_simpl; reflexivity).
       replace (map ioc lw ++ map ioc lw ++ l ++ flat_map (app (map ioc lw)) L1)
          with (flat_map (app (map ioc lw)) (nil :: l :: L1))
-        by (list_simpl ; reflexivity).
+        by (list_simpl; reflexivity).
       refine (IHpi2 _ _ _); reflexivity.
     * rewrite <- ? app_assoc in IHpi2.
       replace (flat_map (cons (ioc A)) (L0 ++ x :: nil) ++
                  ioc A :: ioc A :: l ++ flat_map (cons (ioc A)) L1)
          with (flat_map (cons (ioc A)) (L0 ++ x :: nil :: l :: L1)) in IHpi2
-        by (rewrite ? flat_map_app ; list_simpl ; reflexivity).
+        by (rewrite ? flat_map_app; list_simpl; reflexivity).
       assert (pi2' := IHpi2 _ _ eq_refl).
       list_simpl in pi2'; list_simpl.
-      rewrite 3 app_assoc ; apply co_list_ilr ; list_simpl; assumption.
-- rewrite f in P_cutfree ; inversion P_cutfree.
-- assert (L = nil) as Hnil ; subst.
+      rewrite 3 app_assoc; apply co_list_ilr; list_simpl; assumption.
+- rewrite f in P_cutfree; inversion P_cutfree.
+- assert (L = nil) as Hnil; subst.
   { specialize P_gax_at_l with a.
     rewrite Heq in P_gax_at_l.
     apply Forall_inf_app_r in P_gax_at_l.
     destruct L; inversion P_gax_at_l as [ | ? ? Hat]; [ reflexivity | ].
     inversion Hat. }
-  list_simpl in Heq ; list_simpl ; subst ; apply gax_ir.
+  list_simpl in Heq; list_simpl; subst; apply gax_ir.
 Qed.
 
-Theorem cut_ir_gaxat : forall A l0 l1 l2 C,
+Theorem cut_ir_gaxat A l0 l1 l2 C :
   ill P l0 A -> ill P (l1 ++ A :: l2) C -> ill P (l1 ++ l0 ++ l2) C.
 Proof.
 case_eq (ipcut P); intros P_cutfree.
-{ intros A l0 l1 l2 C pi1 pi2; eapply cut_ir; eassumption. }
+{ intros pi1 pi2; eapply cut_ir; eassumption. }
+revert A l0 l1 l2 C.
 enough (forall c s A l0 l1 l2 C (pi1 : ill P l0 A) (pi2 : ill P (l1 ++ A :: l2) C),
           s = ipsize pi1 + ipsize pi2 -> ifsize A <= c -> ill P (l1 ++ l0 ++ l2) C) as IH
   by (intros A l0 l1 l2 C pi1 pi2; refine (IH _ _ A _ _ _ _ pi1 pi2 _ _); reflexivity).
 induction c as [c IHcut0] using lt_wf_rect.
 assert (forall A, ifsize A < c -> forall l0 l1 l2 C,
           ill P l0 A -> ill P (l1 ++ A :: l2) C -> ill P (l1 ++ l0 ++ l2) C) as IHcut
-  by (intros A Hs l0 l1 l2 C pi1 pi2; refine (IHcut0 _ _ _ _ _ _ _ _ pi1 pi2 _ _);
+  by (intros A' Hs l0' l1' l2' C' pi1 pi2; refine (IHcut0 _ _ _ _ _ _ _ _ pi1 pi2 _ _);
       try reflexivity; assumption);
   clear IHcut0.
 induction s as [s IHsize0] using lt_wf_rect.
@@ -520,17 +519,13 @@ remember (l1 ++ A :: l2) as l; destruct_ill pi2 f X l Hl Hr HP a.
         cbn in Heq ; subst.
       apply Permutation_Type_app_inv in HP.
       revert Hl IHsize; list_simpl; rewrite app_assoc; intros Hl IHsize.
-      rewrite app_assoc; eapply (@cut_oc_comm_left P_cutfree (ipsize pi1)); [ | | reflexivity ].
-      -- list_simpl ; rewrite app_comm_cons ; change (ioc x :: map ioc l7) with (map ioc (x :: l7));
-           rewrite (app_assoc (map ioc l4)) ; rewrite <- map_app.
-         apply (ex_oc_ir _ (l1' ++ x :: l2')); [ | now apply Permutation_Type_elt ].
-         revert Hl IHsize; list_simpl; rewrite app_assoc; intros Hl IHsize; assumption.
-      -- intros lw pi0 Hs'.
-         list_simpl ; rewrite (app_assoc (map ioc l4)) ; rewrite (app_assoc _ (map ioc l7)) ;
-           rewrite <- (app_assoc (map ioc l4)) ; rewrite <- 2 map_app ;
+      rewrite app_assoc; eapply (@cut_oc_comm_left P_cutfree (ipsize pi1)); [ | reflexivity ].
+      intros lw pi0 Hs'.
+      list_simpl; rewrite (app_assoc (map ioc l4)), (app_assoc _ (map ioc l7)),
+                          <- (app_assoc (map ioc l4)), <- 2 map_app;
            apply (ex_oc_ir _ (l1' ++ lw ++ l2')); [ | now apply Permutation_Type_app_middle ].
-         list_simpl ; rewrite app_assoc.
-         refine (IHsize _ _ _ _ _ (oc_irr pi0) Hl _ _); cbn; [ lia | assumption ].
+      list_simpl; rewrite app_assoc.
+      refine (IHsize _ _ _ _ _ (oc_irr pi0) Hl _ _); cbn; [ lia | assumption ].
     * rewrite <- 2 app_assoc.
       eapply ex_oc_ir; [ | eassumption ].
       revert Hl IHsize; cbn; rewrite 2 app_assoc; intros Hl IHsize.
@@ -541,259 +536,259 @@ remember (l1 ++ A :: l2) as l; destruct_ill pi2 f X l Hl Hr HP a.
   trichot_elt_elt_inf_exec Heql.
   + list_simpl.
     apply one_ilr.
-    revert Hl IHsize ; cbn ; rewrite app_assoc ; intros Hl IHsize.
-    rewrite app_assoc ; refine (IHsize _ _ _ _ _ pi1 Hl _ _); lia.
-  + remember (one_ilr _ _ _ Hl) as Hone ; clear HeqHone.
-    remember (ione) as C ; destruct_ill pi1 f X l Hl2 Hr2 HP a ; try inversion HeqC.
+    revert Hl IHsize; cbn; rewrite app_assoc; intros Hl IHsize.
+    rewrite app_assoc; refine (IHsize _ _ _ _ _ pi1 Hl _ _); lia.
+  + remember (one_ilr _ _ _ Hl) as Hone eqn:HeqHone; clear HeqHone.
+    remember (ione) as C; destruct_ill pi1 f X l Hl2 Hr2 HP a; try inversion HeqC.
     * apply (ex_ir (l3 ++ l ++ l4)).
-      -- cbn in IHsize ; refine (IHsize _ _ _ _ _ Hl2 Hone _ _); lia.
-      -- apply PEPermutation_Type_app_head ; apply PEPermutation_Type_app_tail; assumption.
-    * list_simpl ; rewrite app_assoc ; eapply ex_oc_ir; [ | eassumption ].
-      list_simpl ; rewrite (app_assoc l) ; rewrite (app_assoc _ l2) ; rewrite <- (app_assoc l).
-      cbn in IHsize ; refine (IHsize _ _ _ _ _ Hl2 Hone _ _); lia.
+      -- cbn in IHsize; refine (IHsize _ _ _ _ _ Hl2 Hone _ _); lia.
+      -- apply PEPermutation_Type_app_head, PEPermutation_Type_app_tail; assumption.
+    * list_simpl; rewrite app_assoc; eapply ex_oc_ir; [ | eassumption ].
+      list_simpl; rewrite (app_assoc l), (app_assoc _ l2), <- (app_assoc l).
+      cbn in IHsize; refine (IHsize _ _ _ _ _ Hl2 Hone _ _); lia.
     * list_simpl; assumption.
-    * list_simpl ; rewrite app_assoc ; apply one_ilr.
-      list_simpl ; rewrite (app_assoc l1).
-      cbn in IHsize ; refine (IHsize _ _ _ _ _ Hl2 Hone _ _); lia.
-    * list_simpl ; rewrite app_assoc ; apply tens_ilr.
-      list_simpl ; rewrite 2 app_comm_cons ; rewrite (app_assoc l1).
-      cbn in IHsize ; refine (IHsize _ _ _ _ _ Hl2 Hone _ _); lia.
-    * list_simpl ; rewrite app_assoc ; apply lpam_ilr; [ assumption | ].
-      list_simpl ; rewrite app_comm_cons ; rewrite (app_assoc l1).
-      cbn in IHsize ; refine (IHsize _ _ _ _ _ Hr2 Hone _ _); lia.
-    * list_simpl ; rewrite app_assoc ; apply lmap_ilr; [ assumption | ].
-      list_simpl ; rewrite app_comm_cons ; rewrite (app_assoc l1).
-      cbn in IHsize ; refine (IHsize _ _ _ _ _ Hr2 Hone _ _); lia.
-    * list_simpl ; rewrite app_assoc ; apply with_ilr1.
-      list_simpl ; rewrite app_comm_cons ; rewrite (app_assoc l1).
-      cbn in IHsize ; refine (IHsize _ _ _ _ _ Hl2 Hone _ _); lia.
-    * list_simpl ; rewrite app_assoc ; apply with_ilr2.
-      list_simpl ; rewrite app_comm_cons ; rewrite (app_assoc l1).
-      cbn in IHsize ; refine (IHsize _ _ _ _ _ Hl2 Hone _ _); lia.
-    * list_simpl ; rewrite app_assoc ; apply zero_ilr.
-    * list_simpl ; rewrite app_assoc ; apply plus_ilr.
-      -- list_simpl ; rewrite app_comm_cons ; rewrite (app_assoc l1).
-         cbn in IHsize ; refine (IHsize _ _ _ _ _ Hl2 Hone _ _); lia.
-      -- list_simpl ; rewrite app_comm_cons ; rewrite (app_assoc l1).
-         cbn in IHsize ; refine (IHsize _ _ _ _ _ Hr2 Hone _ _); lia.
-    * list_simpl ; rewrite app_assoc ; apply de_ilr.
-      list_simpl ; rewrite app_comm_cons ; rewrite (app_assoc l1).
-      cbn in IHsize ; refine (IHsize _ _ _ _ _ Hl2 Hone _ _); lia.
-    * list_simpl ; rewrite app_assoc ; apply wk_ilr.
-      list_simpl ; rewrite (app_assoc l1).
-      cbn in IHsize ; refine (IHsize _ _ _ _ _ Hl2 Hone _ _); lia.
-    * list_simpl ; rewrite app_assoc ; apply co_ilr.
-      list_simpl ; rewrite 2 app_comm_cons ; rewrite (app_assoc l1).
-      cbn in IHsize ; refine (IHsize _ _ _ _ _ Hl2 Hone _ _); lia.
-    * rewrite f in P_cutfree ; inversion P_cutfree.
-    * exfalso ; assert (Hiq := P_gax_at_r a) ; rewrite H0 in Hiq ; inversion Hiq.
+    * list_simpl; rewrite app_assoc; apply one_ilr.
+      list_simpl; rewrite (app_assoc l1).
+      cbn in IHsize; refine (IHsize _ _ _ _ _ Hl2 Hone _ _); lia.
+    * list_simpl; rewrite app_assoc; apply tens_ilr.
+      list_simpl; rewrite 2 app_comm_cons, (app_assoc l1).
+      cbn in IHsize; refine (IHsize _ _ _ _ _ Hl2 Hone _ _); lia.
+    * list_simpl; rewrite app_assoc; apply lpam_ilr; [ assumption | ].
+      list_simpl; rewrite app_comm_cons, (app_assoc l1).
+      cbn in IHsize; refine (IHsize _ _ _ _ _ Hr2 Hone _ _); lia.
+    * list_simpl; rewrite app_assoc; apply lmap_ilr; [ assumption | ].
+      list_simpl; rewrite app_comm_cons, (app_assoc l1).
+      cbn in IHsize; refine (IHsize _ _ _ _ _ Hr2 Hone _ _); lia.
+    * list_simpl; rewrite app_assoc; apply with_ilr1.
+      list_simpl; rewrite app_comm_cons, (app_assoc l1).
+      cbn in IHsize; refine (IHsize _ _ _ _ _ Hl2 Hone _ _); lia.
+    * list_simpl; rewrite app_assoc; apply with_ilr2.
+      list_simpl; rewrite app_comm_cons, (app_assoc l1).
+      cbn in IHsize; refine (IHsize _ _ _ _ _ Hl2 Hone _ _); lia.
+    * list_simpl; rewrite app_assoc; apply zero_ilr.
+    * list_simpl; rewrite app_assoc; apply plus_ilr.
+      -- list_simpl; rewrite app_comm_cons, (app_assoc l1).
+         cbn in IHsize; refine (IHsize _ _ _ _ _ Hl2 Hone _ _); lia.
+      -- list_simpl; rewrite app_comm_cons, (app_assoc l1).
+         cbn in IHsize; refine (IHsize _ _ _ _ _ Hr2 Hone _ _); lia.
+    * list_simpl; rewrite app_assoc; apply de_ilr.
+      list_simpl; rewrite app_comm_cons, (app_assoc l1).
+      cbn in IHsize; refine (IHsize _ _ _ _ _ Hl2 Hone _ _); lia.
+    * list_simpl; rewrite app_assoc; apply wk_ilr.
+      list_simpl; rewrite (app_assoc l1).
+      cbn in IHsize; refine (IHsize _ _ _ _ _ Hl2 Hone _ _); lia.
+    * list_simpl; rewrite app_assoc; apply co_ilr.
+      list_simpl; rewrite 2 app_comm_cons, (app_assoc l1).
+      cbn in IHsize; refine (IHsize _ _ _ _ _ Hl2 Hone _ _); lia.
+    * rewrite f in P_cutfree; inversion P_cutfree.
+    * exfalso; assert (Hiq := P_gax_at_r a); rewrite H0 in Hiq; inversion Hiq.
   + rewrite 2 app_assoc.
     apply one_ilr.
-    revert Hl IHsize ; list_simpl ; intros Hl IHsize.
+    revert Hl IHsize; list_simpl; intros Hl IHsize.
     refine (IHsize _ _ _ _ _ pi1 Hl _ _); lia.
 - (* tens_irr *)
-  dichot_elt_app_inf_exec Heql ; subst.
-  + rewrite 2 app_assoc ; apply tens_irr; [ | assumption ].
-    revert Hl IHsize ; list_simpl ; intros Hl IHsize.
+  dichot_elt_app_inf_exec Heql; subst.
+  + rewrite 2 app_assoc; apply tens_irr; [ | assumption ].
+    revert Hl IHsize; list_simpl; intros Hl IHsize.
     refine (IHsize _ _ _ _ _ pi1 Hl _ _); lia.
-  + rewrite <- app_assoc ; apply tens_irr; [ assumption | ].
-    revert Hl IHsize ; list_simpl ; intros Hl IHsize.
+  + rewrite <- app_assoc; apply tens_irr; [ assumption | ].
+    revert Hl IHsize; list_simpl; intros Hl IHsize.
     refine (IHsize _ _ _ _ _ pi1 Hr _ _); lia.
 - (* tens_ilr *)
   trichot_elt_elt_inf_exec Heql.
   + list_simpl.
     apply tens_ilr.
-    revert Hl IHsize ; cbn ; rewrite 2 app_comm_cons ; rewrite app_assoc ; intros Hl IHsize.
-    rewrite 2 app_comm_cons ; rewrite app_assoc.
+    revert Hl IHsize; cbn; rewrite 2 app_comm_cons, app_assoc; intros Hl IHsize.
+    rewrite 2 app_comm_cons, app_assoc.
     refine (IHsize _ _ _ _ _ pi1 Hl _ _); lia.
-  + remember (tens_ilr _ _ _ _ _ Hl) as Htens ; clear HeqHtens.
-    remember (itens A0 B) as D ; destruct_ill pi1 f X l Hl2 Hr2 HP a ; try inversion HeqD.
+  + remember (tens_ilr _ _ _ _ _ Hl) as Htens eqn:HeqHtens; clear HeqHtens.
+    remember (itens A0 B) as D; destruct_ill pi1 f X l Hl2 Hr2 HP a; try inversion HeqD.
     * apply (ex_ir (l3 ++ l ++ l4)).
-      -- cbn in IHsize ; refine (IHsize _ _ _ _ _ Hl2 Htens _ _); lia.
-      -- apply PEPermutation_Type_app_head ; apply PEPermutation_Type_app_tail; assumption.
-    * list_simpl ; rewrite app_assoc ; eapply ex_oc_ir; [ | eassumption ].
-      list_simpl ; rewrite (app_assoc l) ; rewrite (app_assoc _ l2) ; rewrite <- (app_assoc l).
-      cbn in IHsize ; refine (IHsize _ _ _ _ _ Hl2 Htens _ _); lia.
-    * list_simpl ; rewrite app_assoc ; apply one_ilr.
-      list_simpl ; rewrite (app_assoc l1).
-      cbn in IHsize ; refine (IHsize _ _ _ _ _ Hl2 Htens _ _); lia.
-    * rewrite <- app_assoc ; rewrite app_assoc.
-      cbn in Hc ; subst ; refine (IHcut _ _ _ _ _ _ Hr2 _); [ lia | ].
-      list_simpl ; refine (IHcut _ _ _ _ _ _ Hl2 Hl); lia.
-    * list_simpl ; rewrite app_assoc ; apply tens_ilr.
-      list_simpl ; rewrite 2 app_comm_cons ; rewrite (app_assoc l1).
-      cbn in IHsize ; refine (IHsize _ _ _ _ _ Hl2 Htens _ _); lia.
-    * list_simpl ; rewrite app_assoc ; apply lpam_ilr; [ assumption | ].
-      list_simpl ; rewrite app_comm_cons ; rewrite (app_assoc l1).
-      cbn in IHsize ; refine (IHsize _ _ _ _ _ Hr2 Htens _ _); lia.
-    * list_simpl ; rewrite app_assoc ; apply lmap_ilr; [ assumption | ].
-      list_simpl ; rewrite app_comm_cons ; rewrite (app_assoc l1).
-      cbn in IHsize ; refine (IHsize _ _ _ _ _ Hr2 Htens _ _); lia.
-    * list_simpl ; rewrite app_assoc ; apply with_ilr1.
-      list_simpl ; rewrite app_comm_cons ; rewrite (app_assoc l1).
-      cbn in IHsize ; refine (IHsize _ _ _ _ _ Hl2 Htens _ _); lia.
-    * list_simpl ; rewrite app_assoc ; apply with_ilr2.
-      list_simpl ; rewrite app_comm_cons ; rewrite (app_assoc l1).
-      cbn in IHsize ; refine (IHsize _ _ _ _ _ Hl2 Htens _ _); lia.
-    * list_simpl ; rewrite app_assoc ; apply zero_ilr.
-    * list_simpl ; rewrite app_assoc ; apply plus_ilr.
-      -- list_simpl ; rewrite app_comm_cons ; rewrite (app_assoc l1).
-         cbn in IHsize ; refine (IHsize _ _ _ _ _ Hl2 Htens _ _); lia.
-      -- list_simpl ; rewrite app_comm_cons ; rewrite (app_assoc l1).
-         cbn in IHsize ; refine (IHsize _ _ _ _ _ Hr2 Htens _ _); lia.
-    * list_simpl ; rewrite app_assoc ; apply de_ilr.
-      list_simpl ; rewrite app_comm_cons ; rewrite (app_assoc l1).
-      cbn in IHsize ; refine (IHsize _ _ _ _ _ Hl2 Htens _ _); lia.
-    * list_simpl ; rewrite app_assoc ; apply wk_ilr.
-      list_simpl ; rewrite (app_assoc l1).
-      cbn in IHsize ; refine (IHsize _ _ _ _ _ Hl2 Htens _ _); lia.
-    * list_simpl ; rewrite app_assoc ; apply co_ilr.
-      list_simpl ; rewrite 2 app_comm_cons ; rewrite (app_assoc l1).
-      cbn in IHsize ; refine (IHsize _ _ _ _ _ Hl2 Htens _ _); lia.
-    * rewrite f in P_cutfree ; inversion P_cutfree.
-    * exfalso ; assert (Hiq := P_gax_at_r a) ; rewrite H0 in Hiq ; inversion Hiq.
+      -- cbn in IHsize; refine (IHsize _ _ _ _ _ Hl2 Htens _ _); lia.
+      -- apply PEPermutation_Type_app_head, PEPermutation_Type_app_tail; assumption.
+    * list_simpl; rewrite app_assoc; eapply ex_oc_ir; [ | eassumption ].
+      list_simpl; rewrite (app_assoc l), (app_assoc _ l2), <- (app_assoc l).
+      cbn in IHsize; refine (IHsize _ _ _ _ _ Hl2 Htens _ _); lia.
+    * list_simpl; rewrite app_assoc ; apply one_ilr.
+      list_simpl; rewrite (app_assoc l1).
+      cbn in IHsize; refine (IHsize _ _ _ _ _ Hl2 Htens _ _); lia.
+    * rewrite <- app_assoc, app_assoc.
+      cbn in Hc; subst; refine (IHcut _ _ _ _ _ _ Hr2 _); [ lia | ].
+      list_simpl; refine (IHcut _ _ _ _ _ _ Hl2 Hl); lia.
+    * list_simpl; rewrite app_assoc; apply tens_ilr.
+      list_simpl; rewrite 2 app_comm_cons, (app_assoc l1).
+      cbn in IHsize; refine (IHsize _ _ _ _ _ Hl2 Htens _ _); lia.
+    * list_simpl; rewrite app_assoc; apply lpam_ilr; [ assumption | ].
+      list_simpl; rewrite app_comm_cons, (app_assoc l1).
+      cbn in IHsize; refine (IHsize _ _ _ _ _ Hr2 Htens _ _); lia.
+    * list_simpl; rewrite app_assoc; apply lmap_ilr; [ assumption | ].
+      list_simpl; rewrite app_comm_cons, (app_assoc l1).
+      cbn in IHsize; refine (IHsize _ _ _ _ _ Hr2 Htens _ _); lia.
+    * list_simpl; rewrite app_assoc; apply with_ilr1.
+      list_simpl; rewrite app_comm_cons, (app_assoc l1).
+      cbn in IHsize; refine (IHsize _ _ _ _ _ Hl2 Htens _ _); lia.
+    * list_simpl; rewrite app_assoc; apply with_ilr2.
+      list_simpl; rewrite app_comm_cons, (app_assoc l1).
+      cbn in IHsize; refine (IHsize _ _ _ _ _ Hl2 Htens _ _); lia.
+    * list_simpl; rewrite app_assoc; apply zero_ilr.
+    * list_simpl; rewrite app_assoc; apply plus_ilr.
+      -- list_simpl; rewrite app_comm_cons, (app_assoc l1).
+         cbn in IHsize; refine (IHsize _ _ _ _ _ Hl2 Htens _ _); lia.
+      -- list_simpl; rewrite app_comm_cons, (app_assoc l1).
+         cbn in IHsize; refine (IHsize _ _ _ _ _ Hr2 Htens _ _); lia.
+    * list_simpl; rewrite app_assoc; apply de_ilr.
+      list_simpl; rewrite app_comm_cons, (app_assoc l1).
+      cbn in IHsize; refine (IHsize _ _ _ _ _ Hl2 Htens _ _); lia.
+    * list_simpl; rewrite app_assoc; apply wk_ilr.
+      list_simpl; rewrite (app_assoc l1).
+      cbn in IHsize; refine (IHsize _ _ _ _ _ Hl2 Htens _ _); lia.
+    * list_simpl; rewrite app_assoc; apply co_ilr.
+      list_simpl; rewrite 2 app_comm_cons, (app_assoc l1).
+      cbn in IHsize; refine (IHsize _ _ _ _ _ Hl2 Htens _ _); lia.
+    * rewrite f in P_cutfree; inversion P_cutfree.
+    * exfalso; assert (Hiq := P_gax_at_r a); rewrite H0 in Hiq; inversion Hiq.
   + rewrite 2 app_assoc.
     apply tens_ilr.
-    revert Hl IHsize ; list_simpl ; intros Hl IHsize.
+    revert Hl IHsize; list_simpl; intros Hl IHsize.
     refine (IHsize _ _ _ _ _ pi1 Hl _ _); lia.
 - (* lpam_irr *)
-  revert Hl IHsize ; list_simpl ; intros Hl IHsize.
+  revert Hl IHsize; list_simpl; intros Hl IHsize.
   apply lpam_irr.
-  list_simpl ; refine (IHsize _ _ _ _ _ pi1 Hl _ _); lia.
+  list_simpl; refine (IHsize _ _ _ _ _ pi1 Hl _ _); lia.
 - (* lpam_ilr *)
-  cbn in IHsize ; trichot_elt_elt_inf_exec Heql.
+  cbn in IHsize; trichot_elt_elt_inf_exec Heql.
   + dichot_elt_app_inf_exec Heql1 ; subst.
-    * list_simpl ; rewrite 2 app_assoc.
+    * list_simpl; rewrite 2 app_assoc.
       apply lpam_ilr; [ | assumption ].
-      list_simpl ; refine (IHsize _ _ _ _ _ pi1 Hl _ _); lia.
-    * list_simpl ; apply lpam_ilr; [ assumption | ].
-      revert Hr IHsize ; rewrite app_comm_cons ; rewrite app_assoc ; intros Hr IHsize.
-      rewrite app_comm_cons ; rewrite app_assoc.
+      list_simpl; refine (IHsize _ _ _ _ _ pi1 Hl _ _); lia.
+    * list_simpl; apply lpam_ilr; [ assumption | ].
+      revert Hr IHsize; rewrite app_comm_cons, app_assoc; intros Hr IHsize.
+      rewrite app_comm_cons, app_assoc.
       refine (IHsize _ _ _ _ _ pi1 Hr _ _); lia.
   + change (S (ipsize Hl + ipsize Hr)) with (ipsize (lpam_ilr _ _ _ _ _ _ Hl Hr)) in IHsize.
-    remember (lpam_ilr _ _ _ _ _ _ Hl Hr) as Hlpam ; clear HeqHlpam.
-    remember (ilpam A0 B) as D ; destruct_ill pi1 f X l Hl2 Hr2 HP a ; try inversion HeqD.
+    remember (lpam_ilr _ _ _ _ _ _ Hl Hr) as Hlpam eqn:HeqHlpam; clear HeqHlpam.
+    remember (ilpam A0 B) as D; destruct_ill pi1 f X l Hl2 Hr2 HP a; try inversion HeqD.
     * apply (ex_ir (l4 ++ l ++ l3 ++ l5)).
-      -- cbn in IHsize ; refine (IHsize _ _ _ _ _ Hl2 Hlpam _ _); lia.
-      -- apply PEPermutation_Type_app_head ; apply PEPermutation_Type_app_tail; assumption.
-    * list_simpl ; rewrite app_assoc ; eapply ex_oc_ir; [ | eassumption ].
-      list_simpl ; rewrite (app_assoc l) ; rewrite (app_assoc _ l2) ; rewrite <- (app_assoc l).
-      cbn in IHsize ; refine (IHsize _ _ _ _ _ Hl2 Hlpam _ _); lia.
-    * list_simpl ; rewrite app_assoc ; apply one_ilr.
-      list_simpl ; rewrite (app_assoc l1).
-      cbn in IHsize ; refine (IHsize _ _ _ _ _ Hl2 Hlpam _ _); lia.
-    * list_simpl ; rewrite app_assoc ; apply tens_ilr.
-      list_simpl ; rewrite 2 app_comm_cons ; rewrite (app_assoc l1).
-      cbn in IHsize ; refine (IHsize _ _ _ _ _ Hl2 Hlpam _ _); lia.
+      -- cbn in IHsize; refine (IHsize _ _ _ _ _ Hl2 Hlpam _ _); lia.
+      -- apply PEPermutation_Type_app_head, PEPermutation_Type_app_tail; assumption.
+    * list_simpl; rewrite app_assoc ; eapply ex_oc_ir; [ | eassumption ].
+      list_simpl; rewrite (app_assoc l), (app_assoc _ l2), <- (app_assoc l).
+      cbn in IHsize; refine (IHsize _ _ _ _ _ Hl2 Hlpam _ _); lia.
+    * list_simpl; rewrite app_assoc; apply one_ilr.
+      list_simpl; rewrite (app_assoc l1).
+      cbn in IHsize; refine (IHsize _ _ _ _ _ Hl2 Hlpam _ _); lia.
+    * list_simpl; rewrite app_assoc; apply tens_ilr.
+      list_simpl; rewrite 2 app_comm_cons, (app_assoc l1).
+      cbn in IHsize; refine (IHsize _ _ _ _ _ Hl2 Hlpam _ _); lia.
     * rewrite app_assoc.
-      cbn in Hc ; subst ; refine (IHcut _ _ _ _ _ _ Hl _); [ lia | ].
-      list_simpl ; change (A0 :: l5) with ((A0 :: nil) ++ l5) ; rewrite (app_assoc l).
+      cbn in Hc; subst; refine (IHcut _ _ _ _ _ _ Hl _); [ lia | ].
+      list_simpl; change (A0 :: l5) with ((A0 :: nil) ++ l5); rewrite (app_assoc l).
       refine (IHcut _ _ _ _ _ _ Hl2 Hr); lia.
-    * list_simpl ; rewrite app_assoc ; apply lpam_ilr; [ assumption | ].
-      list_simpl ; rewrite app_comm_cons ; rewrite (app_assoc l1).
-      cbn in IHsize ; refine (IHsize _ _ _ _ _ Hr2 Hlpam _ _); lia.
-    * list_simpl ; rewrite app_assoc ; apply lmap_ilr; [ assumption | ].
-      list_simpl ; rewrite app_comm_cons ; rewrite (app_assoc l1).
-      cbn in IHsize ; refine (IHsize _ _ _ _ _ Hr2 Hlpam _ _); lia.
-    * list_simpl ; rewrite app_assoc ; apply with_ilr1.
-      list_simpl ; rewrite app_comm_cons ; rewrite (app_assoc l1).
-      cbn in IHsize ; refine (IHsize _ _ _ _ _ Hl2 Hlpam _ _); lia.
-    * list_simpl ; rewrite app_assoc ; apply with_ilr2.
-      list_simpl ; rewrite app_comm_cons ; rewrite (app_assoc l1).
-      cbn in IHsize ; refine (IHsize _ _ _ _ _ Hl2 Hlpam _ _); lia.
-    * list_simpl ; rewrite app_assoc ; apply zero_ilr.
-    * list_simpl ; rewrite app_assoc ; apply plus_ilr.
-      -- list_simpl ; rewrite app_comm_cons ; rewrite (app_assoc l1).
-         cbn in IHsize ; refine (IHsize _ _ _ _ _ Hl2 Hlpam _ _); lia.
-      -- list_simpl ; rewrite app_comm_cons ; rewrite (app_assoc l1).
-         cbn in IHsize ; refine (IHsize _ _ _ _ _ Hr2 Hlpam _ _); lia.
-    * list_simpl ; rewrite app_assoc ; apply de_ilr.
-      list_simpl ; rewrite app_comm_cons ; rewrite (app_assoc l1).
-      cbn in IHsize ; refine (IHsize _ _ _ _ _ Hl2 Hlpam _ _); lia.
-    * list_simpl ; rewrite app_assoc ; apply wk_ilr.
-      list_simpl ; rewrite (app_assoc l1).
-      cbn in IHsize ; refine (IHsize _ _ _ _ _ Hl2 Hlpam _ _); lia.
-    * list_simpl ; rewrite app_assoc ; apply co_ilr.
-      list_simpl ; rewrite 2 app_comm_cons ; rewrite (app_assoc l1).
-      cbn in IHsize ; refine (IHsize _ _ _ _ _ Hl2 Hlpam _ _); lia.
-    * rewrite f in P_cutfree ; inversion P_cutfree.
-    * exfalso ; assert (Hiq := P_gax_at_r a) ; rewrite H0 in Hiq ; inversion Hiq.
-  + rewrite 2 app_assoc ; apply lpam_ilr; [ assumption | ].
-    revert Hr IHsize ; list_simpl ; intros Hr IHsize.
+    * list_simpl; rewrite app_assoc ; apply lpam_ilr; [ assumption | ].
+      list_simpl; rewrite app_comm_cons, (app_assoc l1).
+      cbn in IHsize; refine (IHsize _ _ _ _ _ Hr2 Hlpam _ _); lia.
+    * list_simpl; rewrite app_assoc; apply lmap_ilr; [ assumption | ].
+      list_simpl; rewrite app_comm_cons, (app_assoc l1).
+      cbn in IHsize; refine (IHsize _ _ _ _ _ Hr2 Hlpam _ _); lia.
+    * list_simpl; rewrite app_assoc; apply with_ilr1.
+      list_simpl; rewrite app_comm_cons, (app_assoc l1).
+      cbn in IHsize; refine (IHsize _ _ _ _ _ Hl2 Hlpam _ _); lia.
+    * list_simpl; rewrite app_assoc; apply with_ilr2.
+      list_simpl; rewrite app_comm_cons, (app_assoc l1).
+      cbn in IHsize; refine (IHsize _ _ _ _ _ Hl2 Hlpam _ _); lia.
+    * list_simpl; rewrite app_assoc; apply zero_ilr.
+    * list_simpl; rewrite app_assoc; apply plus_ilr.
+      -- list_simpl; rewrite app_comm_cons, (app_assoc l1).
+         cbn in IHsize; refine (IHsize _ _ _ _ _ Hl2 Hlpam _ _); lia.
+      -- list_simpl; rewrite app_comm_cons, (app_assoc l1).
+         cbn in IHsize; refine (IHsize _ _ _ _ _ Hr2 Hlpam _ _); lia.
+    * list_simpl; rewrite app_assoc; apply de_ilr.
+      list_simpl; rewrite app_comm_cons, (app_assoc l1).
+      cbn in IHsize; refine (IHsize _ _ _ _ _ Hl2 Hlpam _ _); lia.
+    * list_simpl; rewrite app_assoc; apply wk_ilr.
+      list_simpl; rewrite (app_assoc l1).
+      cbn in IHsize; refine (IHsize _ _ _ _ _ Hl2 Hlpam _ _); lia.
+    * list_simpl; rewrite app_assoc; apply co_ilr.
+      list_simpl; rewrite 2 app_comm_cons, (app_assoc l1).
+      cbn in IHsize; refine (IHsize _ _ _ _ _ Hl2 Hlpam _ _); lia.
+    * rewrite f in P_cutfree; inversion P_cutfree.
+    * exfalso; assert (Hiq := P_gax_at_r a); rewrite H0 in Hiq; inversion Hiq.
+  + rewrite 2 app_assoc; apply lpam_ilr; [ assumption | ].
+    revert Hr IHsize; list_simpl; intros Hr IHsize.
     refine (IHsize _ _ _ _ _ pi1 Hr _ _); lia.
 - (* gen_irr *)
   cbn in IHsize.
   apply gen_irr.
-  revert Hl IHsize ; list_simpl ; intros Hl IHsize.
+  revert Hl IHsize; list_simpl; intros Hl IHsize.
   refine (IHsize _ _ _ _ _ pi1 Hl _ _); lia.
 - (* gen_ilr *)
   destruct l1 ; inversion Heql ; subst.
-  + remember (gen_ilr _ _ Hl) as Hgen ; clear HeqHgen.
-    remember (igen A0) as D ; destruct_ill pi1 f X l' Hl2 Hr2 HP a ; try inversion HeqD.
+  + remember (gen_ilr _ _ Hl) as Hgen eqn:HeqHgen; clear HeqHgen.
+    remember (igen A0) as D; destruct_ill pi1 f X l' Hl2 Hr2 HP a; try inversion HeqD.
     * apply (ex_ir (nil ++ l' ++ l2)).
-      -- revert Hgen IHsize ; rewrite <- (app_nil_l _) ; intros Hgen IHsize.
+      -- revert Hgen IHsize; rewrite <- (app_nil_l _); intros Hgen IHsize.
          refine (IHsize _ _ _ _ _ Hl2 Hgen _ _); cbn; [ lia | assumption ].
-      -- apply PEPermutation_Type_app_head ; apply PEPermutation_Type_app_tail; assumption.
-    * rewrite <- ? app_assoc ; rewrite app_assoc ; eapply ex_oc_ir; [ | eassumption ].
+      -- apply PEPermutation_Type_app_head, PEPermutation_Type_app_tail; assumption.
+    * rewrite <- ? app_assoc, app_assoc; eapply ex_oc_ir; [ | eassumption ].
       rewrite <- app_assoc, (app_assoc l'), (app_assoc _ l0), <- (app_assoc l').
-      revert Hgen IHsize ; rewrite <- (app_nil_l _) ; intros Hgen IHsize.
-      refine (IHsize _ _ _ _ _ Hl2 Hgen _ _) ; cbn; [ lia | assumption ].
-    * rewrite <- ? app_assoc ; rewrite app_assoc ; apply one_ilr.
-      list_simpl ; rewrite (app_assoc l1).
-      revert Hgen IHsize ; rewrite <- (app_nil_l _) ; intros Hgen IHsize.
-      refine (IHsize _ _ _ _ _ Hl2 Hgen _ _) ; cbn; [ lia | assumption ].
-    * rewrite <- ? app_assoc ; rewrite app_assoc ; apply tens_ilr.
-      list_simpl ; rewrite 2 app_comm_cons ; rewrite (app_assoc l1).
-      revert Hgen IHsize ; rewrite <- (app_nil_l _) ; intros Hgen IHsize.
-      refine (IHsize _ _ _ _ _ Hl2 Hgen _ _) ; cbn; [ lia | assumption ].
-    * rewrite <- ? app_assoc ; rewrite <- app_comm_cons ; rewrite <- app_assoc ; rewrite app_assoc.
+      revert Hgen IHsize; rewrite <- (app_nil_l _); intros Hgen IHsize.
+      refine (IHsize _ _ _ _ _ Hl2 Hgen _ _); cbn; [ lia | assumption ].
+    * rewrite <- ? app_assoc, app_assoc; apply one_ilr.
+      list_simpl; rewrite (app_assoc l1).
+      revert Hgen IHsize; rewrite <- (app_nil_l _); intros Hgen IHsize.
+      refine (IHsize _ _ _ _ _ Hl2 Hgen _ _); cbn; [ lia | assumption ].
+    * rewrite <- ? app_assoc, app_assoc; apply tens_ilr.
+      list_simpl; rewrite 2 app_comm_cons, (app_assoc l1).
+      revert Hgen IHsize; rewrite <- (app_nil_l _); intros Hgen IHsize.
+      refine (IHsize _ _ _ _ _ Hl2 Hgen _ _); cbn; [ lia | assumption ].
+    * rewrite <- ? app_assoc, <- app_comm_cons, <- app_assoc, app_assoc.
       apply lpam_ilr; [ assumption | ].
-      rewrite <- app_assoc ; rewrite app_comm_cons ; rewrite (app_assoc l1).
-      revert Hgen IHsize ; rewrite <- (app_nil_l _) ; intros Hgen IHsize.
-      refine (IHsize _ _ _ _ _ Hr2 Hgen  _ _) ; cbn; [ lia | assumption ].
-    * subst ; list_simpl ; rewrite <- (app_nil_r _) ; rewrite <- app_assoc.
-      refine (IHcut _ _ _ _ _ _ Hl Hl2) ; cbn; assumption.
-    * rewrite <- ? app_assoc ; rewrite app_assoc ; apply lmap_ilr; [ assumption | ].
-      list_simpl ; rewrite app_comm_cons ; rewrite (app_assoc l1).
-      revert Hgen IHsize ; rewrite <- (app_nil_l _) ; intros Hgen IHsize.
-      refine (IHsize _ _ _ _ _ Hr2 Hgen _ _) ; cbn; [ lia | assumption ].
-    * rewrite <- ? app_assoc ; rewrite app_assoc ; apply with_ilr1.
-      list_simpl ; rewrite app_comm_cons ; rewrite (app_assoc l1).
-      revert Hgen IHsize ; rewrite <- (app_nil_l _) ; intros Hgen IHsize.
-      refine (IHsize _ _ _ _ _ Hl2 Hgen _ _) ; cbn; [ lia | assumption ].
-    * rewrite <- ? app_assoc ; rewrite app_assoc ; apply with_ilr2.
-      list_simpl ; rewrite app_comm_cons ; rewrite (app_assoc l1).
-      revert Hgen IHsize ; rewrite <- (app_nil_l _) ; intros Hgen IHsize.
-      refine (IHsize _ _ _ _ _ Hl2 Hgen _ _) ; cbn; [ lia | assumption ].
-    * rewrite <- ? app_assoc ; rewrite app_assoc ; apply zero_ilr.
-    * rewrite <- ? app_assoc ; rewrite app_assoc ; apply plus_ilr.
-      -- list_simpl ; rewrite app_comm_cons ; rewrite (app_assoc l1).
-         revert Hgen IHsize ; rewrite <- (app_nil_l _) ; intros Hgen IHsize.
-         refine (IHsize _ _ _ _ _ Hl2 Hgen _ _) ; cbn; [ lia | assumption ].
-      -- list_simpl ; rewrite app_comm_cons ; rewrite (app_assoc l1).
-         revert Hgen IHsize ; rewrite <- (app_nil_l _) ; intros Hgen IHsize.
-         refine (IHsize _ _ _ _ _ Hr2 Hgen _ _) ; cbn; [ lia | assumption ].
-    * rewrite <- ? app_assoc ; rewrite app_assoc ; apply de_ilr.
-      list_simpl ; rewrite app_comm_cons ; rewrite (app_assoc l1).
-      revert Hgen IHsize ; rewrite <- (app_nil_l _) ; intros Hgen IHsize.
-      refine (IHsize _ _ _ _ _ Hl2 Hgen _ _) ; cbn; [ lia | assumption ].
-    * rewrite <- ? app_assoc ; rewrite app_assoc ; apply wk_ilr.
-      list_simpl ; rewrite (app_assoc l1).
-      revert Hgen IHsize ; rewrite <- (app_nil_l _) ; intros Hgen IHsize.
-      refine (IHsize _ _ _ _ _ Hl2 Hgen _ _) ; cbn; [ lia | assumption ].
-    * rewrite <- ? app_assoc ; rewrite app_assoc ; apply co_ilr.
-      list_simpl ; rewrite 2 app_comm_cons ; rewrite (app_assoc l1).
-      revert Hgen IHsize ; rewrite <- (app_nil_l _) ; intros Hgen IHsize.
-      refine (IHsize _ _ _ _ _ Hl2 Hgen _ _) ; cbn; [ lia | assumption ].
-    * rewrite f in P_cutfree ; inversion P_cutfree.
-    * exfalso ; assert (Hiq := P_gax_at_r a) ; rewrite H0 in Hiq ; inversion Hiq.
-  + list_simpl ; apply gen_ilr.
-    refine (IHsize _ _ _ _ _ pi1 Hl _ _) ; cbn; [ lia | assumption ].
+      rewrite <- app_assoc, app_comm_cons, (app_assoc l1).
+      revert Hgen IHsize; rewrite <- (app_nil_l _); intros Hgen IHsize.
+      refine (IHsize _ _ _ _ _ Hr2 Hgen  _ _); cbn; [ lia | assumption ].
+    * subst; list_simpl; rewrite <- (app_nil_r _), <- app_assoc.
+      refine (IHcut _ _ _ _ _ _ Hl Hl2); cbn; assumption.
+    * rewrite <- ? app_assoc, app_assoc; apply lmap_ilr; [ assumption | ].
+      list_simpl; rewrite app_comm_cons, (app_assoc l1).
+      revert Hgen IHsize; rewrite <- (app_nil_l _); intros Hgen IHsize.
+      refine (IHsize _ _ _ _ _ Hr2 Hgen _ _); cbn; [ lia | assumption ].
+    * rewrite <- ? app_assoc, app_assoc; apply with_ilr1.
+      list_simpl; rewrite app_comm_cons, (app_assoc l1).
+      revert Hgen IHsize; rewrite <- (app_nil_l _); intros Hgen IHsize.
+      refine (IHsize _ _ _ _ _ Hl2 Hgen _ _); cbn; [ lia | assumption ].
+    * rewrite <- ? app_assoc, app_assoc; apply with_ilr2.
+      list_simpl; rewrite app_comm_cons, (app_assoc l1).
+      revert Hgen IHsize; rewrite <- (app_nil_l _); intros Hgen IHsize.
+      refine (IHsize _ _ _ _ _ Hl2 Hgen _ _); cbn; [ lia | assumption ].
+    * rewrite <- ? app_assoc, app_assoc; apply zero_ilr.
+    * rewrite <- ? app_assoc, app_assoc; apply plus_ilr.
+      -- list_simpl; rewrite app_comm_cons, (app_assoc l1).
+         revert Hgen IHsize; rewrite <- (app_nil_l _); intros Hgen IHsize.
+         refine (IHsize _ _ _ _ _ Hl2 Hgen _ _); cbn; [ lia | assumption ].
+      -- list_simpl; rewrite app_comm_cons, (app_assoc l1).
+         revert Hgen IHsize; rewrite <- (app_nil_l _); intros Hgen IHsize.
+         refine (IHsize _ _ _ _ _ Hr2 Hgen _ _); cbn; [ lia | assumption ].
+    * rewrite <- ? app_assoc, app_assoc; apply de_ilr.
+      list_simpl; rewrite app_comm_cons, (app_assoc l1).
+      revert Hgen IHsize; rewrite <- (app_nil_l _); intros Hgen IHsize.
+      refine (IHsize _ _ _ _ _ Hl2 Hgen _ _); cbn; [ lia | assumption ].
+    * rewrite <- ? app_assoc, app_assoc; apply wk_ilr.
+      list_simpl; rewrite (app_assoc l1).
+      revert Hgen IHsize; rewrite <- (app_nil_l _); intros Hgen IHsize.
+      refine (IHsize _ _ _ _ _ Hl2 Hgen _ _); cbn; [ lia | assumption ].
+    * rewrite <- ? app_assoc, app_assoc; apply co_ilr.
+      list_simpl; rewrite 2 app_comm_cons, (app_assoc l1).
+      revert Hgen IHsize; rewrite <- (app_nil_l _); intros Hgen IHsize.
+      refine (IHsize _ _ _ _ _ Hl2 Hgen _ _); cbn; [ lia | assumption ].
+    * rewrite f in P_cutfree; inversion P_cutfree.
+    * exfalso; assert (Hiq := P_gax_at_r a); rewrite H0 in Hiq; inversion Hiq.
+  + list_simpl; apply gen_ilr.
+    refine (IHsize _ _ _ _ _ pi1 Hl _ _); cbn; [ lia | assumption ].
 - (* lmap_irr *)
   cbn in IHsize.
   apply lmap_irr.
-  revert Hl IHsize ; rewrite app_comm_cons ; intros Hl IHsize.
-  rewrite app_comm_cons ; refine (IHsize _ _ _ _ _ pi1 Hl _ _); [ lia | assumption ].
+  revert Hl IHsize; rewrite app_comm_cons; intros Hl IHsize.
+  rewrite app_comm_cons; refine (IHsize _ _ _ _ _ pi1 Hl _ _); [ lia | assumption ].
 - (* lmap_ilr *)
   cbn in IHsize ; rewrite app_assoc in Heql ; trichot_elt_elt_inf_exec Heql.
   + list_simpl ; apply lmap_ilr; [ assumption | ].
@@ -1150,13 +1145,11 @@ remember (l1 ++ A :: l2) as l; destruct_ill pi2 f X l Hl Hr HP a.
 - (* oc_irr *)
   remember (oc_irr Hl) as Hloc ; rewrite HeqHloc in IHsize ; clear HeqHloc.
   decomp_map_inf Heql; subst; cbn in pi1, IHsize, Hl; list_simpl.
-  eapply (@cut_oc_comm_left P_cutfree (ipsize pi1)); [ | | reflexivity ].
-  + change (ioc x :: map ioc l6) with (map ioc (x :: l6)).
-    rewrite <- map_app; apply oc_irr; assumption.
-  + intros lw Hs' pi.
-    rewrite <- 2 map_app; apply oc_irr.
-    revert Hl IHsize; list_simpl; intros Hl IHsize.
-    refine (IHsize _ _ _ _ _ (oc_irr Hs') Hl _ _); cbn; [ lia | assumption ].
+  eapply (@cut_oc_comm_left P_cutfree (ipsize pi1)); [ | reflexivity ].
+  intros lw Hs' pi.
+  rewrite <- 2 map_app; apply oc_irr.
+  revert Hl IHsize; list_simpl; intros Hl IHsize.
+  refine (IHsize _ _ _ _ _ (oc_irr Hs') Hl _ _); cbn; [ lia | assumption ].
 - (* de_ilr *)
   trichot_elt_elt_inf_exec Heql.
   + list_simpl.
@@ -1164,10 +1157,9 @@ remember (l1 ++ A :: l2) as l; destruct_ill pi2 f X l Hl Hr HP a.
     revert Hl IHsize; cbn; rewrite app_comm_cons, app_assoc; intros Hl IHsize.
     rewrite app_comm_cons, app_assoc.
     refine (IHsize _ _ _ _ _ pi1 Hl _ _); lia.
-  + eapply (@cut_oc_comm_left P_cutfree (ipsize pi1)); [ | | reflexivity ].
-    * apply de_ilr; assumption.
-    * intros lw Hs pi.
-      cbn in Hc; refine (IHsize _ _ _ _ _ Hs Hl _ _); cbn; lia.
+  + eapply (@cut_oc_comm_left P_cutfree (ipsize pi1)); [ | reflexivity ].
+    intros lw Hs pi.
+    cbn in Hc; refine (IHsize _ _ _ _ _ Hs Hl _ _); cbn; lia.
   + rewrite 2 app_assoc.
     apply de_ilr.
     revert Hl IHsize; list_simpl; intros Hl IHsize.
@@ -1179,10 +1171,8 @@ remember (l1 ++ A :: l2) as l; destruct_ill pi2 f X l Hl Hr HP a.
     revert Hl IHsize; cbn; rewrite app_assoc; intros Hl IHsize.
     rewrite app_assoc.
     refine (IHsize _ _ _ _ _ pi1 Hl _ _); lia.
-  + eapply (@cut_oc_comm_left P_cutfree (ipsize pi1)); [ | | reflexivity ].
-    * apply wk_ilr; assumption.
-    * intros lw Hs pi.
-      apply wk_list_ilr; assumption.
+  + eapply (@cut_oc_comm_left P_cutfree (ipsize pi1)); [ | reflexivity ].
+    intros lw Hs pi; apply wk_list_ilr; assumption.
   + rewrite 2 app_assoc.
     apply wk_ilr.
     revert Hl IHsize; list_simpl; intros Hl IHsize.
@@ -1194,17 +1184,15 @@ remember (l1 ++ A :: l2) as l; destruct_ill pi2 f X l Hl Hr HP a.
     revert Hl IHsize ; cbn ; rewrite 2 app_comm_cons, app_assoc ; intros Hl IHsize.
     rewrite 2 app_comm_cons ; rewrite app_assoc.
     refine (IHsize _ _ _ _ _ pi1 Hl _ _); lia.
-  + eapply (@cut_oc_comm_left P_cutfree (ipsize pi1)); [ | | reflexivity ].
-    * apply co_ilr; assumption.
-    * intros lw Hs _.
-      replace (ioc A0 :: ioc A0 :: l4)
-         with (flat_map (cons (ioc A0)) (nil :: l4 :: nil)) in Hl  by (list_simpl ; reflexivity).
-      apply co_list_ilr.
-      replace (map ioc lw ++ map ioc lw ++ l4)
-         with (flat_map (app (map ioc lw)) (nil :: l4 :: nil)) by (list_simpl ; reflexivity).
-      refine (substitution_ioc _ _ _ _ _ _ _ _);
-        list_simpl; try eassumption; [ | reflexivity ].
-      apply IHcut; assumption.
+  + eapply (@cut_oc_comm_left P_cutfree (ipsize pi1)); [ | reflexivity ].
+    intros lw Hs _.
+    replace (ioc A0 :: ioc A0 :: l4)
+       with (flat_map (cons (ioc A0)) (nil :: l4 :: nil)) in Hl  by (list_simpl ; reflexivity).
+    apply co_list_ilr.
+    replace (map ioc lw ++ map ioc lw ++ l4)
+       with (flat_map (app (map ioc lw)) (nil :: l4 :: nil)) by (list_simpl ; reflexivity).
+    refine (substitution_ioc _ _ _ _ _ _ _ _); list_simpl; try eassumption; [ | reflexivity ].
+    apply IHcut; assumption.
   + rewrite 2 app_assoc.
     apply co_ilr.
     revert Hl IHsize ; list_simpl ; intros Hl IHsize.
