yalla/mell_mset.v
@@ -82,10 +82,9 @@ Lemma mell2ll_map_wn l : map mell2ll (map wn l) = map formulas.wn (map mell2ll l
 Proof. induction l as [ | a l IHl ]; [ | cbn; rewrite IHl ]; reflexivity. Qed.
 
 Lemma mell2ll_map_wn_inv l1 l2 : Permutation_Type (map formulas.wn l1) (map mell2ll l2) ->
-  { pl & ((l1 = map mell2ll (fst pl)) * (l2 = map wn (snd pl))
-        * (Permutation_Type (fst pl) (snd pl)))%type }.
+  {'(l1', l2') & l1 = map mell2ll l1' /\ l2 = map wn l2' & Permutation_Type l1' l2' }.
 Proof.
-induction l1 in l2 |- *; intros Heq; destruct l2.
+induction l1 in l2 |- *; intros Heq; destruct l2 as [ | f l2 ].
 - exists (nil, nil); repeat split; reflexivity.
 - apply Permutation_Type_nil in Heq.
   inversion Heq.
@@ -94,14 +93,12 @@ induction l1 in l2 |- *; intros Heq; destruct l2.
   inversion Heq.
 - assert (HP := Heq).
   symmetry in Heq.
-  apply Permutation_Type_vs_cons_inv in Heq.
-  destruct Heq as ((l0 & l3) & Heq).
-  destruct l0.
+  apply Permutation_Type_vs_cons_inv in Heq as [(l0, l3) Heq].
+  destruct l0 as [ | f0 l0 ].
   + cbn in Heq, HP; inversion Heq; subst.
     rewrite H0 in HP.
     apply Permutation_Type_cons_inv in HP.
-    apply IHl1 in HP.
-    destruct HP as ((l1' & l2') & (-> & ->) & HP).
+    apply IHl1 in HP as [(l1', l2') [-> ->] HP].
     destruct f; inversion H0.
     exists (f :: l1', f :: l2'); repeat split.
     apply Permutation_Type_cons; [ reflexivity | assumption ].
@@ -112,12 +109,10 @@ induction l1 in l2 |- *; intros Heq; destruct l2.
     replace (mell2ll f :: map mell2ll l4 ++ map mell2ll l6)
       with (map mell2ll ((f :: l4) ++ l6))
       in HP by (list_simpl; reflexivity).
-    apply IHl1 in HP.
-    destruct HP as ((l1' & l2') & (Heq1 & Heq2) & HP).
-    cbn in Heq1, Heq2, H1, HP; subst.
+    apply IHl1 in HP as [(l1', l2') [-> Heq2] HP].
     destruct x; inversion H1.
     symmetry in Heq2; decomp_map_inf Heq2; subst.
-    exists (x :: l1', x0 :: l1 ++ x :: l2); repeat split.
+    exists (x :: l1', x0 :: l2 ++ x :: l1); repeat split.
     * list_simpl; reflexivity.
     * rewrite app_comm_cons.
       apply Permutation_Type_cons_app; assumption.
@@ -182,29 +177,19 @@ Definition pfrag_mell := @ll_def.mk_pfrag atom  false ll_def.NoAxioms (fun n => 
 
 Lemma mell2mellfrag m : mell m -> inhabited (ll_def.ll pfrag_mell (map mell2ll (elts m))).
 Proof.
-intros pi; induction pi; simpl; rewrite ? map_app;
+intros pi; induction pi;
   try (destruct IHpi as [IHpi]); try (destruct IHpi1 as [IHpi1]); try (destruct IHpi2 as [IHpi2]);
   constructor.
-- apply (ll_def.ex_r (map mell2ll (covar X :: var X :: nil))).
+- cbn; match goal with |- context[if ?b then _ else _] => destruct b end.
   + apply ll_def.ax_r.
-  + symmetry.
-    destruct (Nat.leb
-         (Basics.compose (Basics.compose nattree2nat
-                                         (fun A => fmformulas.form2nattree A)) mell2ll (covar X))
-         (Basics.compose (Basics.compose nattree2nat
-                                         (fun A => fmformulas.form2nattree A)) mell2ll (var X))).
-    * reflexivity.
-    * apply Permutation_Type_swap.
+  + apply (ll_def.ex_r (map mell2ll (covar X :: var X :: nil))); [ apply ll_def.ax_r | ].
+    apply Permutation_Type_swap.
 - apply ll_def.one_r.
 - eapply ll_def.ex_r.
   + apply ll_def.bot_r; eassumption.
   + change (formulas.bot :: map mell2ll (elts m))
       with (map mell2ll (bot :: elts m)).
     apply Permutation_Type_map.
-    rewrite <- (@insert_add border_formula).
-    assert (proj1_sig (fmslist_add bot m) = elts (add bot m)) 
-      as Helt by reflexivity.
-    rewrite Helt.
     symmetry; apply elts_add.
 - eapply ll_def.ex_r.
   + apply ll_def.tens_r.
@@ -219,11 +204,6 @@ intros pi; induction pi; simpl; rewrite ? map_app;
               :: map mell2ll (proj1_sig m2 ++ proj1_sig m1))
       with (map mell2ll (tens A B :: elts m2 ++ elts m1)).
     apply Permutation_Type_map.
-    rewrite <- (@insert_add border_formula).
-    assert (proj1_sig (fmslist_add (tens A B) (sum m1 m2))
-              = elts (add (tens A B) (sum m1 m2)))
-      as Helt by reflexivity.
-    rewrite Helt.
     etransitivity; [ apply Permutation_Type_cons;
                       [ reflexivity | apply Permutation_Type_app_comm ] | ].
     etransitivity; [ apply Permutation_Type_cons;
@@ -232,42 +212,29 @@ intros pi; induction pi; simpl; rewrite ? map_app;
 - eapply ll_def.ex_r.
   + apply ll_def.parr_r.
     assert (Permutation_Type (elts (add A (add B m))) (A :: B :: elts m))
-      as Helt.
+      as Helt%(Permutation_Type_map mell2ll).
     { etransitivity; [ apply elts_add | ].
       apply Permutation_Type_cons, elts_add; reflexivity. }
-    apply (Permutation_Type_map mell2ll) in Helt.
     apply (ll_def.ex_r _ _ IHpi) in Helt.
     cbn in Helt; eassumption.
   + change (formulas.parr (mell2ll A) (mell2ll B) :: map mell2ll (proj1_sig m))
       with (map mell2ll (parr A B :: elts m)).
     apply Permutation_Type_map.
-    rewrite <- (@insert_add border_formula).
-    assert (proj1_sig (fmslist_add (parr A B) m) = elts (add (parr A B) m)) 
-      as Helt by reflexivity.
-    rewrite Helt.
     symmetry; apply elts_add.
 - eapply ll_def.ex_r.
   + apply ll_def.oc_r.
     assert (Permutation_Type (elts (add A (fmmap wn m))) (A :: map wn (elts m)))
-      as Helt.
+      as Helt%(Permutation_Type_map  mell2ll).
     { etransitivity; [ apply elts_add | ].
       apply Permutation_Type_cons, elts_fmmap; reflexivity. }
-    apply (Permutation_Type_map  mell2ll) in Helt.
     apply (ll_def.ex_r _ _ IHpi) in Helt.
     eapply ll_def.ex_r; [ apply Helt | ].
-    cbn.
-    apply Permutation_Type_cons; [ reflexivity | ].
-    rewrite mell2ll_map_wn.
-    apply Permutation_Type_map; reflexivity.
+    cbn; apply Permutation_Type_cons; [ reflexivity | ].
+    rewrite mell2ll_map_wn; apply Permutation_Type_map; reflexivity.
   + rewrite <- mell2ll_map_wn.
     change (formulas.oc (mell2ll A) :: map mell2ll (map wn (proj1_sig m)))
       with (map mell2ll (oc A :: map wn (elts m))).
     apply Permutation_Type_map.
-    rewrite <- (@insert_add border_formula).
-    assert (proj1_sig (fmslist_add (oc A) (fmmap wn m))
-              = elts (add (oc A) (fmmap wn m)))
-      as Helt by reflexivity.
-    rewrite Helt.
     symmetry; etransitivity; [ apply elts_add | ].
     apply Permutation_Type_cons, elts_fmmap; reflexivity.
 - eapply ll_def.ex_r.
@@ -278,39 +245,25 @@ intros pi; induction pi; simpl; rewrite ? map_app;
   + change (formulas.wn (mell2ll A) :: map mell2ll (proj1_sig m))
       with (map mell2ll (wn A :: elts m)).
     apply Permutation_Type_map.
-    rewrite <- (@insert_add border_formula).
-    assert (proj1_sig (fmslist_add (wn A) m) = elts (add (wn A) m)) 
-      as Helt by reflexivity.
-    rewrite Helt.
     symmetry; apply elts_add.
 - eapply ll_def.ex_r.
   + apply (ll_def.wk_r (mell2ll A)); eassumption.
   + change (formulas.wn (mell2ll A) :: map mell2ll (elts m))
       with (map mell2ll (wn A :: elts m)).
     apply Permutation_Type_map.
-    rewrite <- (@insert_add border_formula).
-    assert (proj1_sig (fmslist_add (wn A) m) = elts (add (wn A) m)) 
-      as Helt by reflexivity.
-    rewrite Helt.
     symmetry; apply elts_add.
 - eapply ll_def.ex_r.
   + apply ll_def.co_r.
-    cbn.
     assert (Permutation_Type (elts (add (wn A) (add (wn A) m)))
                              (wn A :: wn A :: elts m))
-      as Helt.
+      as Helt%(Permutation_Type_map mell2ll).
     { etransitivity; [ apply elts_add | ].
       apply Permutation_Type_cons, elts_add; reflexivity. }
-    apply (Permutation_Type_map mell2ll) in Helt.
     apply (ll_def.ex_r _ _ IHpi) in Helt.
     cbn in Helt; eassumption.
   + change (formulas.wn (mell2ll A) :: map mell2ll (proj1_sig m))
       with (map mell2ll (wn A :: elts m)).
     apply Permutation_Type_map.
-    rewrite <- (@insert_add border_formula).
-    assert (proj1_sig (fmslist_add (wn A) m) = elts (add (wn A) m)) 
-      as Helt by reflexivity.
-    rewrite Helt.
     symmetry; apply elts_add.
 Qed.
 
@@ -340,16 +293,14 @@ induction pi in m, HP |- *; subst;
     assert (add (var X) (add (covar X) empty)
           = add (covar X) (add (var X) empty))
       as Hswap by apply add_swap.
-    unfold add in Hswap.
-    cbn in Hswap.
+    unfold add in Hswap; cbn in Hswap.
     rewrite Hswap.
     apply ax_r.
 - apply IHpi.
-  cbn in p.
-  etransitivity; eassumption.
+  transitivity l2; assumption.
 - apply IHpi.
   etransitivity; [ | eassumption ].
-  apply Permutation_Type_app_head,  Permutation_Type_app_tail, Permutation_Type_map; assumption.
+  apply Permutation_Type_app_head, Permutation_Type_app_tail, Permutation_Type_map; assumption.
 - apply Permutation_Type_length_1_inv in HP.
   remember (elts m) as l.
   destruct l; inversion HP.
@@ -466,7 +417,7 @@ induction pi in m, HP |- *; subst;
   apply Permutation_Type_cons_app_inv in HP2.
   rewrite <- map_app in HP2.
   apply mell2ll_map_wn_inv in HP2.
-  destruct HP2 as ((l1' & l2') & (Heq1 & Heq2) & HP); subst.
+  destruct HP2 as [(l1', l2') [-> Heq2] HP].
   rewrite Heq2.
   erewrite list2fm_map.
   apply oc_r, IHpi.
@@ -474,11 +425,9 @@ induction pi in m, HP |- *; subst;
   unfold fmmap.
   etransitivity; [ | symmetry; apply elts_perm ].
   etransitivity; [ | symmetry; apply Permutation_Type_map, elts_add ].
-  simpl; apply Permutation_Type_cons; [ reflexivity | ].
+  rewrite map_cons; apply Permutation_Type_cons; [ reflexivity | ].
   rewrite <- mell2ll_map_wn.
   apply Permutation_Type_map.
-  change (proj1_sig (list2fm (map wn (proj1_sig (list2fm l2')))))
-    with (elts (list2fm (map wn (elts (list2fm l2'))))).
   etransitivity; [ | symmetry; apply elts_perm ].
   apply Permutation_Type_map.
   etransitivity; [ | symmetry; apply elts_perm ]; assumption.
@@ -552,7 +501,7 @@ induction pi in m, HP |- *; subst;
   apply Permutation_Type_cons_app.
   symmetry.
   apply HP2.
-- inversion a.
+- destruct a.
 Qed.
 
 
